\subsection{Rotations in Mass sector for eigenstates {\tt 'EWSB'} } 
\subsubsection{Mass Matrices for Scalars}
\begin{itemize} 
\item {\bf Mass matrix for Higgs}, Basis: \( \left(\rho_1, \rho_2, \rho_S\right), \left(\rho_1, \rho_2, \rho_S\right) \) 
 
\begin{equation} 
m^2_{h} = \left( 
\begin{array}{ccc}
m_{\rho_1\rho_1} &m_{\rho_2\rho_1} &m_{\rho_S\rho_1}\\ 
m_{\rho_1\rho_2} &m_{\rho_2\rho_2} &m_{\rho_S\rho_2}\\ 
m_{\rho_1\rho_S} &m_{\rho_2\rho_S} &m_{\rho_S\rho_S}\end{array} 
\right) 
 \end{equation} 
\begin{align} 
m_{\rho_1\rho_1} &= \frac{1}{4} \Big(12 v_1 v_2 {\Re\Big(\lambda_6\Big)}  + 4 v_S \Big(2 {\Re\Big(\mu_{11}\Big)}  + v_S \Big(2 {\Re\Big(\lambda^{\prime}_4\Big)}  + \lambda^{\prime}_1\Big)\Big) + 6 \lambda_1 v_{1}^{2}  + v_{2}^{2} \Big(2 \Big(\lambda_3 + \lambda_4\Big) + 2 {\Re\Big(\lambda_5\Big)} \Big)\Big) + m^2_{11}\\ 
m_{\rho_1\rho_2} &= \frac{1}{4} \Big(2 \Big(v_1 v_2 \Big(2 \Big(\lambda_3 + \lambda_4\Big) + 2 {\Re\Big(\lambda_5\Big)} \Big) + v_S \Big(2 {\Re\Big(\mu_{12}\Big)}  + 2 {\Re\Big(\mu_{21}\Big)}  + v_S \Big(2 {\Re\Big(\lambda^{\prime}_3\Big)}  + 2 {\Re\Big(\lambda^{\prime}_6\Big)}  + 2 {\Re\Big(\lambda^{\prime}_7\Big)} \Big)\Big)\Big) + 3 \Big(2 v_{1}^{2} {\Re\Big(\lambda_6\Big)}  + 2 v_{2}^{2} {\Re\Big(\lambda_7\Big)} \Big) -4 {\Re\Big(m^2_{12}\Big)} \Big)\\ 
m_{\rho_2\rho_2} &= \frac{1}{2} \Big(2 v_S \Big(2 {\Re\Big(\mu_{22}\Big)}  + v_S \Big(2 {\Re\Big(\lambda^{\prime}_5\Big)}  + \lambda^{\prime}_2\Big)\Big) + 3 \Big(2 v_1 v_2 {\Re\Big(\lambda_7\Big)}  + \lambda_2 v_{2}^{2} \Big) + v_{1}^{2} \Big(\lambda_3 + \lambda_4 + {\Re\Big(\lambda_5\Big)}\Big)\Big) + m^2_{22}\\ 
m_{\rho_1\rho_S} &= \frac{1}{2} \Big(4 v_1 {\Re\Big(\mu_{11}\Big)}  + v_2 \Big(2 {\Re\Big(\mu_{12}\Big)}  + 2 {\Re\Big(\mu_{21}\Big)}  + 2 v_S \Big(2 {\Re\Big(\lambda^{\prime}_6\Big)}  + 2 {\Re\Big(\lambda^{\prime}_7\Big)}  + \lambda^{\prime}_3\Big)\Big) + v_S \Big(2 v_2 \lambda^{{\prime},*}_3  + 4 v_1 \Big(2 {\Re\Big(\lambda^{\prime}_4\Big)}  + \lambda^{\prime}_1\Big)\Big)\Big)\\ 
m_{\rho_2\rho_S} &= v_1 \Big(\frac{1}{2} \Big(2 {\Re\Big(\mu_{21}\Big)}  + 2 v_S \Big(\lambda^{{\prime},*}_6 + \lambda^{{\prime},*}_7\Big) + \mu_{12} + \text{MU12}^*\Big) + v_S \Big(2 {\Re\Big(\lambda^{\prime}_3\Big)}  + \lambda^{\prime}_6 + \lambda^{\prime}_7\Big)\Big) + v_2 \Big(2 {\Re\Big(\mu_{22}\Big)}  + 2 v_S \Big(2 {\Re\Big(\lambda^{\prime}_5\Big)}  + \lambda^{\prime}_2\Big)\Big)\\ 
m_{\rho_S\rho_S} &= +\lambda^{\prime}_1 v_{1}^{2} +\Big(\lambda^{\prime}_2 + \lambda^{\prime}_5\Big)v_{2}^{2} +\frac{1}{2} \Big(v_{S}^{2} \lambda_1''^*  + v_S \Big(2 \mu_{S1}  + \Big(4 \lambda_2''  + 6 \lambda^{\prime\prime}_3  + \lambda_1''\Big)v_S  + 6 \mu_{S2} \Big)\Big)+v_S \Big(2 v_S \lambda_2''^*  + 3 \mu_{S2}^*  + \mu_{S1}^*\Big)\nonumber \\ 
 &+2 \Big(v_{1}^{2} {\Re\Big(\lambda^{\prime}_4\Big)}  + m_{S}^2\Big)+v_2 \Big(v_1 \Big(2 {\Re\Big(\lambda^{\prime}_3\Big)}  + 2 {\Re\Big(\lambda^{\prime}_6\Big)}  + 2 {\Re\Big(\lambda^{\prime}_7\Big)} \Big) + v_2 \lambda^{{\prime},*}_5 \Big)+2 {\Re\Big({m_{S}'}^2\Big)} 
\end{align} 
This matrix is diagonalized by \(Z^H\): 
\begin{equation} 
Z^H m^2_{h} Z^{H,\dagger} = m^{dia}_{2,h} 
\end{equation} 
with 
\begin{align} 
\rho_1 = \sum_{j}Z_{{j 1}}^{H}h_{{j}}\,, \hspace{1cm} 
\rho_2 = \sum_{j}Z_{{j 2}}^{H}h_{{j}}\,, \hspace{1cm} 
\rho_S = \sum_{j}Z_{{j 3}}^{H}h_{{j}}
\end{align} 
\item {\bf Mass matrix for Pseudo-Scalar Higgs}, Basis: \( \left(\eta_1, \eta_2, \eta_S\right), \left(\eta_1, \eta_2, \eta_S\right) \) 
 
\begin{equation} 
m^2_{A^0} = \left( 
\begin{array}{ccc}
m_{\eta_1\eta_1} &m_{\eta_2\eta_1} &m_{\eta_S\eta_1}\\ 
m_{\eta_1\eta_2} &m_{\eta_2\eta_2} &m_{\eta_S\eta_2}\\ 
m_{\eta_1\eta_S} &m_{\eta_2\eta_S} &m_{\eta_S\eta_S}\end{array} 
\right) +  \xi_{Z}m^2(Z) 
 \end{equation} 
\begin{align} 
m_{\eta_1\eta_1} &= \frac{1}{4} \Big(2 \lambda_1 v_{1}^{2}  + 4 \Big(v_1 v_2 {\Re\Big(\lambda_6\Big)}  + v_S \Big(2 {\Re\Big(\mu_{11}\Big)}  + v_S \Big(2 {\Re\Big(\lambda^{\prime}_4\Big)}  + \lambda^{\prime}_1\Big)\Big)\Big) + v_{2}^{2} \Big(2 \Big(\lambda_3 + \lambda_4\Big) -2 {\Re\Big(\lambda_5\Big)} \Big)\Big) + m^2_{11}\\ 
m_{\eta_1\eta_2} &= \frac{1}{4} \Big(2 \Big(2 v_1 v_2 {\Re\Big(\lambda_5\Big)}  + v_S \Big(2 {\Re\Big(\mu_{12}\Big)}  + 2 {\Re\Big(\mu_{21}\Big)}  + v_S \Big(2 {\Re\Big(\lambda^{\prime}_3\Big)}  + 2 {\Re\Big(\lambda^{\prime}_6\Big)}  + 2 {\Re\Big(\lambda^{\prime}_7\Big)} \Big)\Big)\Big) + 2 v_{1}^{2} {\Re\Big(\lambda_6\Big)}  + 2 v_{2}^{2} {\Re\Big(\lambda_7\Big)}  -4 {\Re\Big(m^2_{12}\Big)} \Big)\\ 
m_{\eta_2\eta_2} &= \frac{1}{2} \Big(2 v_1 v_2 {\Re\Big(\lambda_7\Big)}  + 2 v_S \Big(2 {\Re\Big(\mu_{22}\Big)}  + v_S \Big(2 {\Re\Big(\lambda^{\prime}_5\Big)}  + \lambda^{\prime}_2\Big)\Big) + \lambda_2 v_{2}^{2}  + v_{1}^{2} \Big(- {\Re\Big(\lambda_5\Big)}  + \lambda_3 + \lambda_4\Big)\Big) + m^2_{22}\\ 
m_{\eta_1\eta_S} &= -\frac{1}{2} v_2 \Big(-2 {\Re\Big(\mu_{12}\Big)}  + 2 {\Re\Big(\mu_{21}\Big)}  + v_S \Big(-4 {\Re\Big(\lambda^{\prime}_6\Big)}  + 4 {\Re\Big(\lambda^{\prime}_7\Big)} \Big)\Big)\\ 
m_{\eta_2\eta_S} &= \frac{1}{2} v_1 \Big(-2 {\Re\Big(\mu_{12}\Big)}  + 2 {\Re\Big(\mu_{21}\Big)}  + v_S \Big(-4 {\Re\Big(\lambda^{\prime}_6\Big)}  + 4 {\Re\Big(\lambda^{\prime}_7\Big)} \Big)\Big)\\ 
m_{\eta_S\eta_S} &= +2 m_{S}^2 +\Big(- \lambda^{\prime}_4  + \lambda^{\prime}_1\Big)v_{1}^{2} +\frac{1}{2} \Big(- v_{S}^{2} \lambda_1''^*  - v_S \Big(-2 \lambda^{\prime\prime}_3 v_S  + 2 \mu_{S1}  -2 \mu_{S2}  + \lambda_1'' v_S \Big)\Big)+v_S \Big(- \mu_{S1}^*  + \mu_{S2}^*\Big)\nonumber \\ 
 &+v_{2}^{2} \Big(-2 {\Re\Big(\lambda^{\prime}_5\Big)}  + \lambda^{\prime}_2\Big)+v_1 \Big(- v_1 \lambda^{{\prime},*}_4  + v_2 \Big(2 {\Re\Big(\lambda^{\prime}_3\Big)}  -2 {\Re\Big(\lambda^{\prime}_6\Big)}  -2 {\Re\Big(\lambda^{\prime}_7\Big)} \Big)\Big)-2 {\Re\Big({m_{S}'}^2\Big)} 
\end{align} 
Gauge fixing contributions: 
\begin{equation} 
m^2 (\xi_{Z}) = \left( 
\begin{array}{ccc}
m_{\eta_1\eta_1} &m_{\eta_2\eta_1} &0\\ 
m_{\eta_1\eta_2} &m_{\eta_2\eta_2} &0\\ 
0 &0 &0\end{array} 
\right) 
 \end{equation} 
\begin{align} 
m_{\eta_1\eta_1} &= \frac{1}{4} v_{1}^{2} \Big(g_1 \sin\Theta_W   + g_2 \cos\Theta_W  \Big)^{2} \\ 
m_{\eta_1\eta_2} &= \frac{1}{4} v_1 v_2 \Big(g_1 \sin\Theta_W   + g_2 \cos\Theta_W  \Big)^{2} \\ 
m_{\eta_2\eta_2} &= \frac{1}{4} v_{2}^{2} \Big(g_1 \sin\Theta_W   + g_2 \cos\Theta_W  \Big)^{2} 
\end{align} 
This matrix is diagonalized by \(Z^A\): 
\begin{equation} 
Z^A m^2_{A^0} Z^{A,\dagger} = m^{dia}_{2,A^0} 
\end{equation} 
with 
\begin{align} 
\eta_1 = \sum_{j}Z_{{j 1}}^{A}A^0_{{j}}\,, \hspace{1cm} 
\eta_2 = \sum_{j}Z_{{j 2}}^{A}A^0_{{j}}\,, \hspace{1cm} 
\eta_S = \sum_{j}Z_{{j 3}}^{A}A^0_{{j}}
\end{align} 
\item {\bf Mass matrix for Charged Higgs}, Basis: \( \left(\chi_1^{\pm,*}, \chi_2^{\pm,*}\right), \left(\chi_1^\pm, \chi_2^\pm\right) \) 
 
\begin{equation} 
m^2_{H^-} = \left( 
\begin{array}{cc}
m_{\chi_1^{\pm,*}\chi_1^\pm} &m^*_{\chi_2^{\pm,*}\chi_1^\pm}\\ 
m_{\chi_1^{\pm,*}\chi_2^\pm} &m_{\chi_2^{\pm,*}\chi_2^\pm}\end{array} 
\right) +  \xi_{W^-}m^2(W^-) 
 \end{equation} 
\begin{align} 
m_{\chi_1^{\pm,*}\chi_1^\pm} &= \frac{1}{2} \Big(2 v_S \Big(\Big(\lambda^{\prime}_1 + \lambda^{\prime}_4\Big)v_S  + \mu_{11}\Big) + \lambda_1 v_{1}^{2}  + \lambda_3 v_{2}^{2} \Big) + v_1 v_2 {\Re\Big(\lambda_6\Big)}  + v_S \Big(v_S \lambda^{{\prime},*}_4  + \mu_{11}^*\Big) + m^2_{11}\\ 
m_{\chi_1^{\pm,*}\chi_2^\pm} &= \frac{1}{2} \Big(-2 m^2_{12}  + 2 v_S \Big(v_S \Big(\lambda^{\prime}_3 + \lambda^{\prime}_6 + \lambda^{{\prime},*}_7\Big) + \mu_{12} + \mu_{21}^*\Big) + \lambda_6 v_{1}^{2}  + \lambda_7 v_{2}^{2}  + v_1 v_2 \Big(\lambda_4 + \lambda_5^*\Big)\Big)\\ 
m_{\chi_2^{\pm,*}\chi_2^\pm} &= \frac{1}{2} \Big(2 v_S \Big(\Big(\lambda^{\prime}_2 + \lambda^{\prime}_5\Big)v_S  + \mu_{22}\Big) + \lambda_2 v_{2}^{2}  + \lambda_3 v_{1}^{2} \Big) + v_1 v_2 {\Re\Big(\lambda_7\Big)}  + v_S \Big(v_S \lambda^{{\prime},*}_5  + \mu_{22}^*\Big) + m^2_{22}
\end{align} 
Gauge fixing contributions: 
\begin{equation} 
m^2 (\xi_{W^-}) = \left( 
\begin{array}{cc}
\frac{1}{4} g_{2}^{2} v_{1}^{2}  &\frac{1}{4} g_{2}^{2} v_1 v_2 \\ 
\frac{1}{4} g_{2}^{2} v_1 v_2  &\frac{1}{4} g_{2}^{2} v_{2}^{2} \end{array} 
\right) 
 \end{equation} 
This matrix is diagonalized by \(Z^+\): 
\begin{equation} 
Z^+ m^2_{H^-} Z^{+,\dagger} = m^{dia}_{2,H^-} 
\end{equation} 
with 
\begin{align} 
\chi_1^\pm = \sum_{j}Z_{{j 1}}^{+}H^+_{{j}}\,, \hspace{1cm} 
\chi_2^\pm = \sum_{j}Z_{{j 2}}^{+}H^+_{{j}}
\end{align} 
\end{itemize} 
