\begin{align} 
\frac{\partial V}{\partial \rho_1} &= \frac{1}{4} \Big(v_{2}^{3} \lambda_7^* +v_1 \Big(4 \Big(v_{S}^{2} \lambda^{{\prime},*}_4  + v_S \mu_{11}^*  + m^2_{11}\Big) + v_{2}^{2} \lambda_5^* \Big)\nonumber \\ 
 &+2 \Big(\lambda_1 v_{1}^{3}  + v_{S}^{2} \Big(2 \Big(\lambda^{\prime}_1 + \lambda^{\prime}_4\Big)v_1  + v_2 \Big(\lambda^{\prime}_3 + \lambda^{\prime}_6 + \lambda^{\prime}_7 + \lambda^{{\prime},*}_6\Big)\Big) + v_S \Big(2 \mu_{11} v_1  + v_2 \Big(\mu_{12} + \mu_{21} + \mu_{12}^*\Big)\Big)\Big)\nonumber \\ 
 &+v_2 \Big(2 \Big(v_{S}^{2} \Big(\lambda^{{\prime},*}_3 + \lambda^{{\prime},*}_7\Big) + v_S \mu_{21}^* \Big) + 3 v_{1}^{2} \Big(\lambda_6 + \lambda_6^*\Big) -4 {\Re\Big(m^2_{12}\Big)}  + v_2 \Big(\Big(2 \Big(\lambda_3 + \lambda_4\Big) + \lambda_5\Big)v_1  + \lambda_7 v_2 \Big)\Big)\Big)\\ 
\frac{\partial V}{\partial \rho_2} &= \frac{1}{4} \Big(v_{1}^{3} \Big(\lambda_6 + \lambda_6^*\Big)+2 \Big(v_{S}^{2} \Big(2 \Big(\lambda^{\prime}_2 + \lambda^{\prime}_5\Big)v_2  + v_1 \Big(\lambda^{\prime}_3 + \lambda^{\prime}_6 + \lambda^{\prime}_7 + \lambda^{{\prime},*}_3 + \lambda^{{\prime},*}_6 + \lambda^{{\prime},*}_7\Big)\Big) + v_S \Big(2 \mu_{22} v_2  + v_1 \Big(\mu_{12} + \mu_{21} + \mu_{21}^*\Big)\Big)\Big)\nonumber \\ 
 &+v_2 \Big(2 \lambda_2 v_{2}^{2}  + 3 \lambda_7 v_1 v_2  + 4 \Big(v_{S}^{2} \lambda^{{\prime},*}_5  + v_S \mu_{22}^*  + m^2_{22}\Big) + v_{1}^{2} \Big(2 \Big(\lambda_3 + \lambda_4\Big) + \lambda_5 + \lambda_5^*\Big)\Big)\nonumber \\ 
 &+v_1 \Big(2 v_S \mu_{12}^*  + 3 v_{2}^{2} \lambda_7^*  -4 {\Re\Big(m^2_{12}\Big)} \Big)\Big)\\ 
\frac{\partial V}{\partial \rho_S} &= \frac{1}{6} \Big(3 \Big(v_{1}^{2} \Big(\mu_{11} + \mu_{11}^*\Big) + v_{2}^{2} \mu_{22}^*  + v_2 \Big(\mu_{22} v_2  + v_1 \Big(\mu_{12} + \mu_{21} + \mu_{12}^* + \mu_{21}^*\Big)\Big) + v_{S}^{2} \Big(\mu_{S1} + \mu_{S1}^*\Big)\Big)+v_{S}^{3} \Big(6 \lambda^{\prime\prime}_3  + 8 {\Re\Big(\lambda_2''\Big)}  + \lambda_1'' + \lambda_1''^*\Big)\nonumber \\ 
 &+v_S \Big(12 v_1 v_2 {\Re\Big(\lambda^{\prime}_3\Big)}  + 6 \Big(2 m_{S}^2  + v_{1}^{2} \Big(\lambda^{\prime}_1 + \lambda^{\prime}_4 + \lambda^{{\prime},*}_4\Big) + v_1 v_2 \Big(\lambda^{\prime}_6 + \lambda^{\prime}_7 + \lambda^{{\prime},*}_6 + \lambda^{{\prime},*}_7\Big) + v_{2}^{2} \Big(\lambda^{\prime}_2 + \lambda^{\prime}_5 + \lambda^{{\prime},*}_5\Big) + {m_{S}'}^2 + {m_{S}'}^{2,*}\Big)\Big)\nonumber \\ 
 &+18 v_{S}^{2} {\Re\Big(\mu_{S2}\Big)} \Big)
\end{align} 
