\begin{center} 
\begin{fmffile}{Diagrams/FeynDia6} 
\fmfframe(20,20)(20,20){ 
\begin{fmfgraph*}(75,75) 
\fmfleft{l1,l2}
\fmfright{r1,r2}
\fmf{dashes}{l1,v1}
\fmf{dashes}{r1,v1}
\fmf{dashes}{r2,v1}
\fmf{dashes}{l2,v1}
\fmflabel{$A^0_{{i}}$}{l1}
\fmflabel{$A^0_{{j}}$}{r1}
\fmflabel{$A^0_{{k}}$}{r2}
\fmflabel{$A^0_{{l}}$}{l2}
\end{fmfgraph*}} 
\end{fmffile} 
\end{center}  
\begin{align} 
 &-\frac{i}{2} \Big(2 Z_{{i 3}}^{A} \Big(Z_{{j 2}}^{A} \Big(Z_{{k 3}}^{A} \Big(2 \Big(- \lambda^{{\prime},*}_5  - \lambda^{\prime}_5  + \lambda^{\prime}_2\Big)Z_{{l 2}}^{A}  + \Big(- \lambda^{{\prime},*}_6  - \lambda^{\prime}_6  - \lambda^{{\prime},*}_7  - \lambda^{\prime}_7  + \lambda^{\prime}_3 + \lambda^{{\prime},*}_3\Big)Z_{{l 1}}^{A} \Big)\nonumber \\ 
 &+\Big(2 \Big(- \lambda^{{\prime},*}_5  - \lambda^{\prime}_5  + \lambda^{\prime}_2\Big)Z_{{k 2}}^{A}  + \Big(- \lambda^{{\prime},*}_6  - \lambda^{\prime}_6  - \lambda^{{\prime},*}_7  - \lambda^{\prime}_7  + \lambda^{\prime}_3 + \lambda^{{\prime},*}_3\Big)Z_{{k 1}}^{A} \Big)Z_{{l 3}}^{A} \Big)\nonumber \\ 
 &+Z_{{j 1}}^{A} \Big(Z_{{k 3}}^{A} \Big(2 \Big(- \lambda^{{\prime},*}_4  - \lambda^{\prime}_4  + \lambda^{\prime}_1\Big)Z_{{l 1}}^{A}  + \Big(- \lambda^{{\prime},*}_6  - \lambda^{\prime}_6  - \lambda^{{\prime},*}_7  - \lambda^{\prime}_7  + \lambda^{\prime}_3 + \lambda^{{\prime},*}_3\Big)Z_{{l 2}}^{A} \Big)\nonumber \\ 
 &+\Big(2 \Big(- \lambda^{{\prime},*}_4  - \lambda^{\prime}_4  + \lambda^{\prime}_1\Big)Z_{{k 1}}^{A}  + \Big(- \lambda^{{\prime},*}_6  - \lambda^{\prime}_6  - \lambda^{{\prime},*}_7  - \lambda^{\prime}_7  + \lambda^{\prime}_3 + \lambda^{{\prime},*}_3\Big)Z_{{k 2}}^{A} \Big)Z_{{l 3}}^{A} \Big)\nonumber \\ 
 &+Z_{{j 3}}^{A} \Big(Z_{{k 2}}^{A} \Big(2 \Big(- \lambda^{{\prime},*}_5  - \lambda^{\prime}_5  + \lambda^{\prime}_2\Big)Z_{{l 2}}^{A}  + \Big(- \lambda^{{\prime},*}_6  - \lambda^{\prime}_6  - \lambda^{{\prime},*}_7  - \lambda^{\prime}_7  + \lambda^{\prime}_3 + \lambda^{{\prime},*}_3\Big)Z_{{l 1}}^{A} \Big)\nonumber \\ 
 &+Z_{{k 1}}^{A} \Big(2 \Big(- \lambda^{{\prime},*}_4  - \lambda^{\prime}_4  + \lambda^{\prime}_1\Big)Z_{{l 1}}^{A}  + \Big(- \lambda^{{\prime},*}_6  - \lambda^{\prime}_6  - \lambda^{{\prime},*}_7  - \lambda^{\prime}_7  + \lambda^{\prime}_3 + \lambda^{{\prime},*}_3\Big)Z_{{l 2}}^{A} \Big)\nonumber \\ 
 &+\Big(-4 \lambda_2''  -4 \lambda_2''^*  + 6 \lambda^{\prime\prime}_3  + \lambda_1'' + \lambda_1''^*\Big)Z_{{k 3}}^{A} Z_{{l 3}}^{A} \Big)\Big)\nonumber \\ 
 &+Z_{{i 2}}^{A} \Big(2 Z_{{j 3}}^{A} \Big(Z_{{k 3}}^{A} \Big(2 \Big(- \lambda^{{\prime},*}_5  - \lambda^{\prime}_5  + \lambda^{\prime}_2\Big)Z_{{l 2}}^{A}  + \Big(- \lambda^{{\prime},*}_6  - \lambda^{\prime}_6  - \lambda^{{\prime},*}_7  - \lambda^{\prime}_7  + \lambda^{\prime}_3 + \lambda^{{\prime},*}_3\Big)Z_{{l 1}}^{A} \Big)\nonumber \\ 
 &+\Big(2 \Big(- \lambda^{{\prime},*}_5  - \lambda^{\prime}_5  + \lambda^{\prime}_2\Big)Z_{{k 2}}^{A}  + \Big(- \lambda^{{\prime},*}_6  - \lambda^{\prime}_6  - \lambda^{{\prime},*}_7  - \lambda^{\prime}_7  + \lambda^{\prime}_3 + \lambda^{{\prime},*}_3\Big)Z_{{k 1}}^{A} \Big)Z_{{l 3}}^{A} \Big)\nonumber \\ 
 &+Z_{{j 2}}^{A} \Big(3 Z_{{k 2}}^{A} \Big(2 \lambda_2 Z_{{l 2}}^{A}  + \Big(\lambda_7 + \lambda_7^*\Big)Z_{{l 1}}^{A} \Big)+Z_{{k 1}}^{A} \Big(\Big(2 \lambda_3  + 2 \lambda_4  + \lambda_5 + \lambda_5^*\Big)Z_{{l 1}}^{A}  + 3 \Big(\lambda_7 + \lambda_7^*\Big)Z_{{l 2}}^{A} \Big)\nonumber \\ 
 &+4 \Big(- \lambda^{{\prime},*}_5  - \lambda^{\prime}_5  + \lambda^{\prime}_2\Big)Z_{{k 3}}^{A} Z_{{l 3}}^{A} \Big)\nonumber \\ 
 &+Z_{{j 1}}^{A} \Big(Z_{{k 1}}^{A} \Big(\Big(2 \lambda_3  + 2 \lambda_4  + \lambda_5 + \lambda_5^*\Big)Z_{{l 2}}^{A}  + 3 \Big(\lambda_6 + \lambda_6^*\Big)Z_{{l 1}}^{A} \Big)+Z_{{k 2}}^{A} \Big(\Big(2 \lambda_3  + 2 \lambda_4  + \lambda_5 + \lambda_5^*\Big)Z_{{l 1}}^{A}  + 3 \Big(\lambda_7 + \lambda_7^*\Big)Z_{{l 2}}^{A} \Big)\nonumber \\ 
 &+2 \Big(- \lambda^{{\prime},*}_6  - \lambda^{\prime}_6  - \lambda^{{\prime},*}_7  - \lambda^{\prime}_7  + \lambda^{\prime}_3 + \lambda^{{\prime},*}_3\Big)Z_{{k 3}}^{A} Z_{{l 3}}^{A} \Big)\Big)\nonumber \\ 
 &+Z_{{i 1}}^{A} \Big(2 Z_{{j 3}}^{A} \Big(Z_{{k 3}}^{A} \Big(2 \Big(- \lambda^{{\prime},*}_4  - \lambda^{\prime}_4  + \lambda^{\prime}_1\Big)Z_{{l 1}}^{A}  + \Big(- \lambda^{{\prime},*}_6  - \lambda^{\prime}_6  - \lambda^{{\prime},*}_7  - \lambda^{\prime}_7  + \lambda^{\prime}_3 + \lambda^{{\prime},*}_3\Big)Z_{{l 2}}^{A} \Big)\nonumber \\ 
 &+\Big(2 \Big(- \lambda^{{\prime},*}_4  - \lambda^{\prime}_4  + \lambda^{\prime}_1\Big)Z_{{k 1}}^{A}  + \Big(- \lambda^{{\prime},*}_6  - \lambda^{\prime}_6  - \lambda^{{\prime},*}_7  - \lambda^{\prime}_7  + \lambda^{\prime}_3 + \lambda^{{\prime},*}_3\Big)Z_{{k 2}}^{A} \Big)Z_{{l 3}}^{A} \Big)\nonumber \\ 
 &+Z_{{j 1}}^{A} \Big(Z_{{k 2}}^{A} \Big(\Big(2 \lambda_3  + 2 \lambda_4  + \lambda_5 + \lambda_5^*\Big)Z_{{l 2}}^{A}  + 3 \Big(\lambda_6 + \lambda_6^*\Big)Z_{{l 1}}^{A} \Big)+3 Z_{{k 1}}^{A} \Big(2 \lambda_1 Z_{{l 1}}^{A}  + \Big(\lambda_6 + \lambda_6^*\Big)Z_{{l 2}}^{A} \Big)\nonumber \\ 
 &+4 \Big(- \lambda^{{\prime},*}_4  - \lambda^{\prime}_4  + \lambda^{\prime}_1\Big)Z_{{k 3}}^{A} Z_{{l 3}}^{A} \Big)\nonumber \\ 
 &+Z_{{j 2}}^{A} \Big(Z_{{k 1}}^{A} \Big(\Big(2 \lambda_3  + 2 \lambda_4  + \lambda_5 + \lambda_5^*\Big)Z_{{l 2}}^{A}  + 3 \Big(\lambda_6 + \lambda_6^*\Big)Z_{{l 1}}^{A} \Big)+Z_{{k 2}}^{A} \Big(\Big(2 \lambda_3  + 2 \lambda_4  + \lambda_5 + \lambda_5^*\Big)Z_{{l 1}}^{A}  + 3 \Big(\lambda_7 + \lambda_7^*\Big)Z_{{l 2}}^{A} \Big)\nonumber \\ 
 &+2 \Big(- \lambda^{{\prime},*}_6  - \lambda^{\prime}_6  - \lambda^{{\prime},*}_7  - \lambda^{\prime}_7  + \lambda^{\prime}_3 + \lambda^{{\prime},*}_3\Big)Z_{{k 3}}^{A} Z_{{l 3}}^{A} \Big)\Big)\Big)\end{align} 
\hrule 
\begin{center} 
\begin{fmffile}{Diagrams/FeynDia7} 
\fmfframe(20,20)(20,20){ 
\begin{fmfgraph*}(75,75) 
\fmfleft{l1,l2}
\fmfright{r1,r2}
\fmf{dashes}{l1,v1}
\fmf{dashes}{r1,v1}
\fmf{dashes}{r2,v1}
\fmf{dashes}{l2,v1}
\fmflabel{$A^0_{{i}}$}{l1}
\fmflabel{$A^0_{{j}}$}{r1}
\fmflabel{$A^0_{{k}}$}{r2}
\fmflabel{$h_{{l}}$}{l2}
\end{fmfgraph*}} 
\end{fmffile} 
\end{center}  
\begin{align} 
 &\frac{1}{2} \Big(2 Z_{{i 3}}^{A} \Big(Z_{{j 2}}^{A} \Big(\Big(- \lambda^{{\prime},*}_3  - \lambda^{\prime}_6  - \lambda^{{\prime},*}_7  + \lambda^{\prime}_3 + \lambda^{\prime}_7 + \lambda^{{\prime},*}_6\Big)Z_{{k 3}}^{A} Z_{{l 1}}^{H} \nonumber \\ 
 &+\Big(2 \Big(- \lambda^{{\prime},*}_5  + \lambda^{\prime}_5\Big)Z_{{k 2}}^{A}  + \Big(- \lambda^{{\prime},*}_6  - \lambda^{{\prime},*}_7  + \lambda^{\prime}_6 + \lambda^{\prime}_7\Big)Z_{{k 1}}^{A} \Big)Z_{{l 3}}^{H} \Big)\nonumber \\ 
 &+Z_{{j 1}}^{A} \Big(\Big(- \lambda^{\prime}_3  - \lambda^{{\prime},*}_6  - \lambda^{\prime}_7  + \lambda^{\prime}_6 + \lambda^{{\prime},*}_3 + \lambda^{{\prime},*}_7\Big)Z_{{k 3}}^{A} Z_{{l 2}}^{H} \nonumber \\ 
 &+\Big(2 \Big(- \lambda^{{\prime},*}_4  + \lambda^{\prime}_4\Big)Z_{{k 1}}^{A}  + \Big(- \lambda^{{\prime},*}_6  - \lambda^{{\prime},*}_7  + \lambda^{\prime}_6 + \lambda^{\prime}_7\Big)Z_{{k 2}}^{A} \Big)Z_{{l 3}}^{H} \Big)\nonumber \\ 
 &+Z_{{j 3}}^{A} \Big(\Big(- \lambda^{{\prime},*}_3  - \lambda^{\prime}_6  - \lambda^{{\prime},*}_7  + \lambda^{\prime}_3 + \lambda^{\prime}_7 + \lambda^{{\prime},*}_6\Big)Z_{{k 2}}^{A} Z_{{l 1}}^{H} +\Big(- \lambda^{\prime}_3  - \lambda^{{\prime},*}_6  - \lambda^{\prime}_7  + \lambda^{\prime}_6 + \lambda^{{\prime},*}_3 + \lambda^{{\prime},*}_7\Big)Z_{{k 1}}^{A} Z_{{l 2}}^{H} \nonumber \\ 
 &+\Big(-2 \lambda_2''^*  + 2 \lambda_2''  - \lambda_1''  + \lambda_1''^*\Big)Z_{{k 3}}^{A} Z_{{l 3}}^{H} \Big)\Big)\nonumber \\ 
 &+Z_{{i 2}}^{A} \Big(2 Z_{{j 3}}^{A} \Big(\Big(- \lambda^{{\prime},*}_3  - \lambda^{\prime}_6  - \lambda^{{\prime},*}_7  + \lambda^{\prime}_3 + \lambda^{\prime}_7 + \lambda^{{\prime},*}_6\Big)Z_{{k 3}}^{A} Z_{{l 1}}^{H} \nonumber \\ 
 &+\Big(2 \Big(- \lambda^{{\prime},*}_5  + \lambda^{\prime}_5\Big)Z_{{k 2}}^{A}  + \Big(- \lambda^{{\prime},*}_6  - \lambda^{{\prime},*}_7  + \lambda^{\prime}_6 + \lambda^{\prime}_7\Big)Z_{{k 1}}^{A} \Big)Z_{{l 3}}^{H} \Big)\nonumber \\ 
 &+Z_{{j 2}}^{A} \Big(3 \Big(- \lambda_7^*  + \lambda_7\Big)Z_{{k 2}}^{A} Z_{{l 1}}^{H}  + 4 \Big(- \lambda^{{\prime},*}_5  + \lambda^{\prime}_5\Big)Z_{{k 3}}^{A} Z_{{l 3}}^{H}  + Z_{{k 1}}^{A} \Big(\Big(- \lambda_5  + \lambda_5^*\Big)Z_{{l 1}}^{H}  + \Big(- \lambda_7  + \lambda_7^*\Big)Z_{{l 2}}^{H} \Big)\Big)\nonumber \\ 
 &+Z_{{j 1}}^{A} \Big(Z_{{k 1}}^{A} \Big(\Big(- \lambda_5^*  + \lambda_5\Big)Z_{{l 2}}^{H}  + \Big(- \lambda_6^*  + \lambda_6\Big)Z_{{l 1}}^{H} \Big)+Z_{{k 2}}^{A} \Big(\Big(- \lambda_5  + \lambda_5^*\Big)Z_{{l 1}}^{H}  + \Big(- \lambda_7  + \lambda_7^*\Big)Z_{{l 2}}^{H} \Big)\nonumber \\ 
 &+2 \Big(- \lambda^{{\prime},*}_6  - \lambda^{{\prime},*}_7  + \lambda^{\prime}_6 + \lambda^{\prime}_7\Big)Z_{{k 3}}^{A} Z_{{l 3}}^{H} \Big)\Big)\nonumber \\ 
 &+Z_{{i 1}}^{A} \Big(-2 Z_{{j 3}}^{A} \Big(\Big(- \lambda^{{\prime},*}_3  - \lambda^{\prime}_6  - \lambda^{{\prime},*}_7  + \lambda^{\prime}_3 + \lambda^{\prime}_7 + \lambda^{{\prime},*}_6\Big)Z_{{k 3}}^{A} Z_{{l 2}}^{H} \nonumber \\ 
 &+\Big(-2 \Big(- \lambda^{{\prime},*}_4  + \lambda^{\prime}_4\Big)Z_{{k 1}}^{A}  + \Big(- \lambda^{\prime}_6  - \lambda^{\prime}_7  + \lambda^{{\prime},*}_6 + \lambda^{{\prime},*}_7\Big)Z_{{k 2}}^{A} \Big)Z_{{l 3}}^{H} \Big)\nonumber \\ 
 &+Z_{{j 1}}^{A} \Big(3 \Big(- \lambda_6  + \lambda_6^*\Big)Z_{{k 1}}^{A} Z_{{l 2}}^{H}  + 4 \Big(- \lambda^{{\prime},*}_4  + \lambda^{\prime}_4\Big)Z_{{k 3}}^{A} Z_{{l 3}}^{H}  + Z_{{k 2}}^{A} \Big(\Big(- \lambda_5^*  + \lambda_5\Big)Z_{{l 2}}^{H}  + \Big(- \lambda_6^*  + \lambda_6\Big)Z_{{l 1}}^{H} \Big)\Big)\nonumber \\ 
 &+Z_{{j 2}}^{A} \Big(Z_{{k 1}}^{A} \Big(\Big(- \lambda_5^*  + \lambda_5\Big)Z_{{l 2}}^{H}  + \Big(- \lambda_6^*  + \lambda_6\Big)Z_{{l 1}}^{H} \Big)+Z_{{k 2}}^{A} \Big(\Big(- \lambda_5  + \lambda_5^*\Big)Z_{{l 1}}^{H}  + \Big(- \lambda_7  + \lambda_7^*\Big)Z_{{l 2}}^{H} \Big)\nonumber \\ 
 &+2 \Big(- \lambda^{{\prime},*}_6  - \lambda^{{\prime},*}_7  + \lambda^{\prime}_6 + \lambda^{\prime}_7\Big)Z_{{k 3}}^{A} Z_{{l 3}}^{H} \Big)\Big)\Big)\end{align} 
\hrule 
\begin{center} 
\begin{fmffile}{Diagrams/FeynDia8} 
\fmfframe(20,20)(20,20){ 
\begin{fmfgraph*}(75,75) 
\fmfleft{l1,l2}
\fmfright{r1,r2}
\fmf{dashes}{l1,v1}
\fmf{dashes}{r1,v1}
\fmf{dashes}{r2,v1}
\fmf{dashes}{l2,v1}
\fmflabel{$A^0_{{i}}$}{l1}
\fmflabel{$A^0_{{j}}$}{r1}
\fmflabel{$h_{{k}}$}{r2}
\fmflabel{$h_{{l}}$}{l2}
\end{fmfgraph*}} 
\end{fmffile} 
\end{center}  
\begin{align} 
 &-\frac{i}{2} \Big(Z_{{i 2}}^{A} \Big(-2 \Big(- \lambda^{{\prime},*}_7  - \lambda^{\prime}_7  + \lambda^{\prime}_6 + \lambda^{{\prime},*}_6\Big)Z_{{j 3}}^{A} \Big(Z_{{k 1}}^{H} Z_{{l 3}}^{H}  + Z_{{k 3}}^{H} Z_{{l 1}}^{H} \Big)\nonumber \\ 
 &+Z_{{j 2}}^{A} \Big(Z_{{k 2}}^{H} \Big(2 \lambda_2 Z_{{l 2}}^{H}  + \Big(\lambda_7 + \lambda_7^*\Big)Z_{{l 1}}^{H} \Big)+Z_{{k 1}}^{H} \Big(\Big(2 \lambda_3  + 2 \lambda_4  - \lambda_5  - \lambda_5^* \Big)Z_{{l 1}}^{H}  + \Big(\lambda_7 + \lambda_7^*\Big)Z_{{l 2}}^{H} \Big)\nonumber \\ 
 &+4 \Big(\lambda^{\prime}_2 + \lambda^{\prime}_5 + \lambda^{{\prime},*}_5\Big)Z_{{k 3}}^{H} Z_{{l 3}}^{H} \Big)\nonumber \\ 
 &+Z_{{j 1}}^{A} \Big(Z_{{k 1}}^{H} \Big(\Big(\lambda_5 + \lambda_5^*\Big)Z_{{l 2}}^{H}  + \Big(\lambda_6 + \lambda_6^*\Big)Z_{{l 1}}^{H} \Big)+Z_{{k 2}}^{H} \Big(\Big(\lambda_5 + \lambda_5^*\Big)Z_{{l 1}}^{H}  + \Big(\lambda_7 + \lambda_7^*\Big)Z_{{l 2}}^{H} \Big)\nonumber \\ 
 &+2 \Big(\lambda^{\prime}_3 + \lambda^{\prime}_6 + \lambda^{\prime}_7 + \lambda^{{\prime},*}_3 + \lambda^{{\prime},*}_6 + \lambda^{{\prime},*}_7\Big)Z_{{k 3}}^{H} Z_{{l 3}}^{H} \Big)\Big)\nonumber \\ 
 &+Z_{{i 1}}^{A} \Big(2 \Big(- \lambda^{{\prime},*}_7  - \lambda^{\prime}_7  + \lambda^{\prime}_6 + \lambda^{{\prime},*}_6\Big)Z_{{j 3}}^{A} \Big(Z_{{k 2}}^{H} Z_{{l 3}}^{H}  + Z_{{k 3}}^{H} Z_{{l 2}}^{H} \Big)\nonumber \\ 
 &+Z_{{j 1}}^{A} \Big(Z_{{k 2}}^{H} \Big(\Big(2 \lambda_3  + 2 \lambda_4  - \lambda_5  - \lambda_5^* \Big)Z_{{l 2}}^{H}  + \Big(\lambda_6 + \lambda_6^*\Big)Z_{{l 1}}^{H} \Big)+Z_{{k 1}}^{H} \Big(2 \lambda_1 Z_{{l 1}}^{H}  + \Big(\lambda_6 + \lambda_6^*\Big)Z_{{l 2}}^{H} \Big)\nonumber \\ 
 &+4 \Big(\lambda^{\prime}_1 + \lambda^{\prime}_4 + \lambda^{{\prime},*}_4\Big)Z_{{k 3}}^{H} Z_{{l 3}}^{H} \Big)\nonumber \\ 
 &+Z_{{j 2}}^{A} \Big(Z_{{k 1}}^{H} \Big(\Big(\lambda_5 + \lambda_5^*\Big)Z_{{l 2}}^{H}  + \Big(\lambda_6 + \lambda_6^*\Big)Z_{{l 1}}^{H} \Big)+Z_{{k 2}}^{H} \Big(\Big(\lambda_5 + \lambda_5^*\Big)Z_{{l 1}}^{H}  + \Big(\lambda_7 + \lambda_7^*\Big)Z_{{l 2}}^{H} \Big)\nonumber \\ 
 &+2 \Big(\lambda^{\prime}_3 + \lambda^{\prime}_6 + \lambda^{\prime}_7 + \lambda^{{\prime},*}_3 + \lambda^{{\prime},*}_6 + \lambda^{{\prime},*}_7\Big)Z_{{k 3}}^{H} Z_{{l 3}}^{H} \Big)\Big)\nonumber \\ 
 &+2 Z_{{i 3}}^{A} \Big(Z_{{j 3}}^{A} \Big(Z_{{k 2}}^{H} \Big(2 \Big(- \lambda^{{\prime},*}_5  - \lambda^{\prime}_5  + \lambda^{\prime}_2\Big)Z_{{l 2}}^{H}  + \Big(- \lambda^{{\prime},*}_6  - \lambda^{\prime}_6  - \lambda^{{\prime},*}_7  - \lambda^{\prime}_7  + \lambda^{\prime}_3 + \lambda^{{\prime},*}_3\Big)Z_{{l 1}}^{H} \Big)\nonumber \\ 
 &+Z_{{k 1}}^{H} \Big(2 \Big(- \lambda^{{\prime},*}_4  - \lambda^{\prime}_4  + \lambda^{\prime}_1\Big)Z_{{l 1}}^{H}  + \Big(- \lambda^{{\prime},*}_6  - \lambda^{\prime}_6  - \lambda^{{\prime},*}_7  - \lambda^{\prime}_7  + \lambda^{\prime}_3 + \lambda^{{\prime},*}_3\Big)Z_{{l 2}}^{H} \Big)\nonumber \\ 
 &- \Big(-2 \lambda^{\prime\prime}_3  + \lambda_1'' + \lambda_1''^*\Big)Z_{{k 3}}^{H} Z_{{l 3}}^{H} \Big)\nonumber \\ 
 &- \Big(- \lambda^{{\prime},*}_7  - \lambda^{\prime}_7  + \lambda^{\prime}_6 + \lambda^{{\prime},*}_6\Big)\Big(- Z_{{j 1}}^{A} \Big(Z_{{k 2}}^{H} Z_{{l 3}}^{H}  + Z_{{k 3}}^{H} Z_{{l 2}}^{H} \Big) + Z_{{j 2}}^{A} \Big(Z_{{k 1}}^{H} Z_{{l 3}}^{H}  + Z_{{k 3}}^{H} Z_{{l 1}}^{H} \Big)\Big)\Big)\Big)\end{align} 
\hrule 
\begin{center} 
\begin{fmffile}{Diagrams/FeynDia9} 
\fmfframe(20,20)(20,20){ 
\begin{fmfgraph*}(75,75) 
\fmfleft{l1,l2}
\fmfright{r1,r2}
\fmf{dashes}{l1,v1}
\fmf{dashes}{r1,v1}
\fmf{scalar}{r2,v1}
\fmf{scalar}{v1,l2}
\fmflabel{$A^0_{{i}}$}{l1}
\fmflabel{$A^0_{{j}}$}{r1}
\fmflabel{$H^-_{{k}}$}{r2}
\fmflabel{$H^+_{{l}}$}{l2}
\end{fmfgraph*}} 
\end{fmffile} 
\end{center}  
\begin{align} 
 &-\frac{i}{2} \Big(4 Z_{{i 3}}^{A} Z_{{j 3}}^{A} \Big(- Z_{{k 2}}^{+} \Big(\Big(- \lambda^{\prime}_2  + \lambda^{\prime}_5 + \lambda^{{\prime},*}_5\Big)Z_{{l 2}}^{+}  + \Big(- \lambda^{{\prime},*}_3  + \lambda^{\prime}_7 + \lambda^{{\prime},*}_6\Big)Z_{{l 1}}^{+} \Big)\nonumber \\ 
 &+Z_{{k 1}}^{+} \Big(\Big(- \lambda^{{\prime},*}_4  - \lambda^{\prime}_4  + \lambda^{\prime}_1\Big)Z_{{l 1}}^{+}  + \Big(- \lambda^{\prime}_6  - \lambda^{{\prime},*}_7  + \lambda^{\prime}_3\Big)Z_{{l 2}}^{+} \Big)\Big)\nonumber \\ 
 &+Z_{{i 2}}^{A} \Big(2 Z_{{j 2}}^{A} \Big(Z_{{k 1}}^{+} \Big(\lambda_3 Z_{{l 1}}^{+}  + \lambda_7 Z_{{l 2}}^{+} \Big) + Z_{{k 2}}^{+} \Big(\lambda_2 Z_{{l 2}}^{+}  + \lambda_7^* Z_{{l 1}}^{+} \Big)\Big)\nonumber \\ 
 &+Z_{{j 1}}^{A} \Big(Z_{{k 1}}^{+} \Big(\Big(\lambda_4 + \lambda_5^*\Big)Z_{{l 2}}^{+}  + \Big(\lambda_6 + \lambda_6^*\Big)Z_{{l 1}}^{+} \Big) + Z_{{k 2}}^{+} \Big(\Big(\lambda_4 + \lambda_5\Big)Z_{{l 1}}^{+}  + \Big(\lambda_7 + \lambda_7^*\Big)Z_{{l 2}}^{+} \Big)\Big)\Big)\nonumber \\ 
 &+Z_{{i 1}}^{A} \Big(2 Z_{{j 1}}^{A} \Big(Z_{{k 1}}^{+} \Big(\lambda_1 Z_{{l 1}}^{+}  + \lambda_6 Z_{{l 2}}^{+} \Big) + Z_{{k 2}}^{+} \Big(\lambda_3 Z_{{l 2}}^{+}  + \lambda_6^* Z_{{l 1}}^{+} \Big)\Big)\nonumber \\ 
 &+Z_{{j 2}}^{A} \Big(Z_{{k 1}}^{+} \Big(\Big(\lambda_4 + \lambda_5^*\Big)Z_{{l 2}}^{+}  + \Big(\lambda_6 + \lambda_6^*\Big)Z_{{l 1}}^{+} \Big) + Z_{{k 2}}^{+} \Big(\Big(\lambda_4 + \lambda_5\Big)Z_{{l 1}}^{+}  + \Big(\lambda_7 + \lambda_7^*\Big)Z_{{l 2}}^{+} \Big)\Big)\Big)\Big)\end{align} 
\hrule 
\begin{center} 
\begin{fmffile}{Diagrams/FeynDia10} 
\fmfframe(20,20)(20,20){ 
\begin{fmfgraph*}(75,75) 
\fmfleft{l1,l2}
\fmfright{r1,r2}
\fmf{dashes}{l1,v1}
\fmf{dashes}{r1,v1}
\fmf{dashes}{r2,v1}
\fmf{dashes}{l2,v1}
\fmflabel{$A^0_{{i}}$}{l1}
\fmflabel{$h_{{j}}$}{r1}
\fmflabel{$h_{{k}}$}{r2}
\fmflabel{$h_{{l}}$}{l2}
\end{fmfgraph*}} 
\end{fmffile} 
\end{center}  
\begin{align} 
 &\frac{1}{2} \Big(2 Z_{{i 3}}^{A} \Big(Z_{{j 2}}^{H} \Big(Z_{{k 3}}^{H} \Big(2 \Big(- \lambda^{{\prime},*}_5  + \lambda^{\prime}_5\Big)Z_{{l 2}}^{H}  + \Big(- \lambda^{{\prime},*}_6  - \lambda^{{\prime},*}_7  + \lambda^{\prime}_6 + \lambda^{\prime}_7\Big)Z_{{l 1}}^{H} \Big)\nonumber \\ 
 &+\Big(2 \Big(- \lambda^{{\prime},*}_5  + \lambda^{\prime}_5\Big)Z_{{k 2}}^{H}  + \Big(- \lambda^{{\prime},*}_6  - \lambda^{{\prime},*}_7  + \lambda^{\prime}_6 + \lambda^{\prime}_7\Big)Z_{{k 1}}^{H} \Big)Z_{{l 3}}^{H} \Big)\nonumber \\ 
 &+Z_{{j 1}}^{H} \Big(Z_{{k 3}}^{H} \Big(2 \Big(- \lambda^{{\prime},*}_4  + \lambda^{\prime}_4\Big)Z_{{l 1}}^{H}  + \Big(- \lambda^{{\prime},*}_6  - \lambda^{{\prime},*}_7  + \lambda^{\prime}_6 + \lambda^{\prime}_7\Big)Z_{{l 2}}^{H} \Big)\nonumber \\ 
 &+\Big(2 \Big(- \lambda^{{\prime},*}_4  + \lambda^{\prime}_4\Big)Z_{{k 1}}^{H}  + \Big(- \lambda^{{\prime},*}_6  - \lambda^{{\prime},*}_7  + \lambda^{\prime}_6 + \lambda^{\prime}_7\Big)Z_{{k 2}}^{H} \Big)Z_{{l 3}}^{H} \Big)\nonumber \\ 
 &+Z_{{j 3}}^{H} \Big(Z_{{k 2}}^{H} \Big(2 \Big(- \lambda^{{\prime},*}_5  + \lambda^{\prime}_5\Big)Z_{{l 2}}^{H}  + \Big(- \lambda^{{\prime},*}_6  - \lambda^{{\prime},*}_7  + \lambda^{\prime}_6 + \lambda^{\prime}_7\Big)Z_{{l 1}}^{H} \Big)\nonumber \\ 
 &+Z_{{k 1}}^{H} \Big(2 \Big(- \lambda^{{\prime},*}_4  + \lambda^{\prime}_4\Big)Z_{{l 1}}^{H}  + \Big(- \lambda^{{\prime},*}_6  - \lambda^{{\prime},*}_7  + \lambda^{\prime}_6 + \lambda^{\prime}_7\Big)Z_{{l 2}}^{H} \Big)+\Big(-2 \lambda_2''^*  + 2 \lambda_2''  - \lambda_1''^*  + \lambda_1''\Big)Z_{{k 3}}^{H} Z_{{l 3}}^{H} \Big)\Big)\nonumber \\ 
 &+Z_{{i 1}}^{A} \Big(Z_{{j 1}}^{H} \Big(\Big(- \lambda_6  + \lambda_6^*\Big)Z_{{k 1}}^{H} Z_{{l 2}}^{H}  + Z_{{k 2}}^{H} \Big(\Big(- \lambda_5^*  + \lambda_5\Big)Z_{{l 2}}^{H}  + \Big(- \lambda_6  + \lambda_6^*\Big)Z_{{l 1}}^{H} \Big)\Big)\nonumber \\ 
 &-2 \Big(- \lambda^{{\prime},*}_3  - \lambda^{{\prime},*}_6  - \lambda^{\prime}_7  + \lambda^{\prime}_3 + \lambda^{\prime}_6 + \lambda^{{\prime},*}_7\Big)Z_{{j 3}}^{H} \Big(Z_{{k 2}}^{H} Z_{{l 3}}^{H}  + Z_{{k 3}}^{H} Z_{{l 2}}^{H} \Big)\nonumber \\ 
 &+Z_{{j 2}}^{H} \Big(Z_{{k 1}}^{H} \Big(\Big(- \lambda_5^*  + \lambda_5\Big)Z_{{l 2}}^{H}  + \Big(- \lambda_6  + \lambda_6^*\Big)Z_{{l 1}}^{H} \Big)+Z_{{k 2}}^{H} \Big(3 \Big(- \lambda_7  + \lambda_7^*\Big)Z_{{l 2}}^{H}  + \Big(- \lambda_5^*  + \lambda_5\Big)Z_{{l 1}}^{H} \Big)\nonumber \\ 
 &+2 \Big(- \lambda^{\prime}_3  - \lambda^{\prime}_6  - \lambda^{{\prime},*}_7  + \lambda^{\prime}_7 + \lambda^{{\prime},*}_3 + \lambda^{{\prime},*}_6\Big)Z_{{k 3}}^{H} Z_{{l 3}}^{H} \Big)\Big)\nonumber \\ 
 &+Z_{{i 2}}^{A} \Big(Z_{{j 2}}^{H} \Big(\Big(- \lambda_7^*  + \lambda_7\Big)Z_{{k 2}}^{H} Z_{{l 1}}^{H}  + Z_{{k 1}}^{H} \Big(\Big(- \lambda_5  + \lambda_5^*\Big)Z_{{l 1}}^{H}  + \Big(- \lambda_7^*  + \lambda_7\Big)Z_{{l 2}}^{H} \Big)\Big)\nonumber \\ 
 &+2 \Big(- \lambda^{{\prime},*}_3  - \lambda^{{\prime},*}_6  - \lambda^{\prime}_7  + \lambda^{\prime}_3 + \lambda^{\prime}_6 + \lambda^{{\prime},*}_7\Big)Z_{{j 3}}^{H} \Big(Z_{{k 1}}^{H} Z_{{l 3}}^{H}  + Z_{{k 3}}^{H} Z_{{l 1}}^{H} \Big)\nonumber \\ 
 &+Z_{{j 1}}^{H} \Big(Z_{{k 1}}^{H} \Big(3 \Big(- \lambda_6^*  + \lambda_6\Big)Z_{{l 1}}^{H}  + \Big(- \lambda_5  + \lambda_5^*\Big)Z_{{l 2}}^{H} \Big)+Z_{{k 2}}^{H} \Big(\Big(- \lambda_5  + \lambda_5^*\Big)Z_{{l 1}}^{H}  + \Big(- \lambda_7^*  + \lambda_7\Big)Z_{{l 2}}^{H} \Big)\nonumber \\ 
 &+2 \Big(- \lambda^{{\prime},*}_3  - \lambda^{{\prime},*}_6  - \lambda^{\prime}_7  + \lambda^{\prime}_3 + \lambda^{\prime}_6 + \lambda^{{\prime},*}_7\Big)Z_{{k 3}}^{H} Z_{{l 3}}^{H} \Big)\Big)\Big)\end{align} 
\hrule 
\begin{center} 
\begin{fmffile}{Diagrams/FeynDia11} 
\fmfframe(20,20)(20,20){ 
\begin{fmfgraph*}(75,75) 
\fmfleft{l1,l2}
\fmfright{r1,r2}
\fmf{dashes}{l1,v1}
\fmf{dashes}{r1,v1}
\fmf{scalar}{r2,v1}
\fmf{scalar}{v1,l2}
\fmflabel{$A^0_{{i}}$}{l1}
\fmflabel{$h_{{j}}$}{r1}
\fmflabel{$H^-_{{k}}$}{r2}
\fmflabel{$H^+_{{l}}$}{l2}
\end{fmfgraph*}} 
\end{fmffile} 
\end{center}  
\begin{align} 
 &\frac{1}{2} \Big(Z_{{i 2}}^{A} Z_{{j 1}}^{H} \Big(Z_{{k 1}}^{+} \Big(\Big(- \lambda_4  + \lambda_5^*\Big)Z_{{l 2}}^{+}  + \Big(- \lambda_6^*  + \lambda_6\Big)Z_{{l 1}}^{+} \Big) + Z_{{k 2}}^{+} \Big(\Big(- \lambda_5  + \lambda_4\Big)Z_{{l 1}}^{+}  + \Big(- \lambda_7^*  + \lambda_7\Big)Z_{{l 2}}^{+} \Big)\Big)\nonumber \\ 
 &+Z_{{i 1}}^{A} Z_{{j 2}}^{H} \Big(Z_{{k 1}}^{+} \Big(\Big(- \lambda_5^*  + \lambda_4\Big)Z_{{l 2}}^{+}  + \Big(- \lambda_6  + \lambda_6^*\Big)Z_{{l 1}}^{+} \Big) + Z_{{k 2}}^{+} \Big(\Big(- \lambda_4  + \lambda_5\Big)Z_{{l 1}}^{+}  + \Big(- \lambda_7  + \lambda_7^*\Big)Z_{{l 2}}^{+} \Big)\Big)\nonumber \\ 
 &+4 Z_{{i 3}}^{A} Z_{{j 3}}^{H} \Big(Z_{{k 1}}^{+} \Big(\Big(- \lambda^{{\prime},*}_4  + \lambda^{\prime}_4\Big)Z_{{l 1}}^{+}  + \Big(- \lambda^{{\prime},*}_7  + \lambda^{\prime}_6\Big)Z_{{l 2}}^{+} \Big) + Z_{{k 2}}^{+} \Big(\Big(- \lambda^{{\prime},*}_5  + \lambda^{\prime}_5\Big)Z_{{l 2}}^{+}  + \Big(- \lambda^{{\prime},*}_6  + \lambda^{\prime}_7\Big)Z_{{l 1}}^{+} \Big)\Big)\Big)\end{align} 
\hrule 
\begin{center} 
\begin{fmffile}{Diagrams/FeynDia12} 
\fmfframe(20,20)(20,20){ 
\begin{fmfgraph*}(75,75) 
\fmfleft{l1,l2}
\fmfright{r1,r2}
\fmf{dashes}{l1,v1}
\fmf{dashes}{r1,v1}
\fmf{dashes}{r2,v1}
\fmf{dashes}{l2,v1}
\fmflabel{$h_{{i}}$}{l1}
\fmflabel{$h_{{j}}$}{r1}
\fmflabel{$h_{{k}}$}{r2}
\fmflabel{$h_{{l}}$}{l2}
\end{fmfgraph*}} 
\end{fmffile} 
\end{center}  
\begin{align} 
 &-\frac{i}{2} \Big(2 Z_{{i 3}}^{H} \Big(Z_{{j 2}}^{H} \Big(Z_{{k 3}}^{H} \Big(2 \Big(\lambda^{\prime}_2 + \lambda^{\prime}_5 + \lambda^{{\prime},*}_5\Big)Z_{{l 2}}^{H}  + \Big(\lambda^{\prime}_3 + \lambda^{\prime}_6 + \lambda^{\prime}_7 + \lambda^{{\prime},*}_3 + \lambda^{{\prime},*}_6 + \lambda^{{\prime},*}_7\Big)Z_{{l 1}}^{H} \Big)\nonumber \\ 
 &+\Big(2 \Big(\lambda^{\prime}_2 + \lambda^{\prime}_5 + \lambda^{{\prime},*}_5\Big)Z_{{k 2}}^{H}  + \Big(\lambda^{\prime}_3 + \lambda^{\prime}_6 + \lambda^{\prime}_7 + \lambda^{{\prime},*}_3 + \lambda^{{\prime},*}_6 + \lambda^{{\prime},*}_7\Big)Z_{{k 1}}^{H} \Big)Z_{{l 3}}^{H} \Big)\nonumber \\ 
 &+Z_{{j 1}}^{H} \Big(Z_{{k 3}}^{H} \Big(2 \Big(\lambda^{\prime}_1 + \lambda^{\prime}_4 + \lambda^{{\prime},*}_4\Big)Z_{{l 1}}^{H}  + \Big(\lambda^{\prime}_3 + \lambda^{\prime}_6 + \lambda^{\prime}_7 + \lambda^{{\prime},*}_3 + \lambda^{{\prime},*}_6 + \lambda^{{\prime},*}_7\Big)Z_{{l 2}}^{H} \Big)\nonumber \\ 
 &+\Big(2 \Big(\lambda^{\prime}_1 + \lambda^{\prime}_4 + \lambda^{{\prime},*}_4\Big)Z_{{k 1}}^{H}  + \Big(\lambda^{\prime}_3 + \lambda^{\prime}_6 + \lambda^{\prime}_7 + \lambda^{{\prime},*}_3 + \lambda^{{\prime},*}_6 + \lambda^{{\prime},*}_7\Big)Z_{{k 2}}^{H} \Big)Z_{{l 3}}^{H} \Big)\nonumber \\ 
 &+Z_{{j 3}}^{H} \Big(Z_{{k 2}}^{H} \Big(2 \Big(\lambda^{\prime}_2 + \lambda^{\prime}_5 + \lambda^{{\prime},*}_5\Big)Z_{{l 2}}^{H}  + \Big(\lambda^{\prime}_3 + \lambda^{\prime}_6 + \lambda^{\prime}_7 + \lambda^{{\prime},*}_3 + \lambda^{{\prime},*}_6 + \lambda^{{\prime},*}_7\Big)Z_{{l 1}}^{H} \Big)\nonumber \\ 
 &+Z_{{k 1}}^{H} \Big(2 \Big(\lambda^{\prime}_1 + \lambda^{\prime}_4 + \lambda^{{\prime},*}_4\Big)Z_{{l 1}}^{H}  + \Big(\lambda^{\prime}_3 + \lambda^{\prime}_6 + \lambda^{\prime}_7 + \lambda^{{\prime},*}_3 + \lambda^{{\prime},*}_6 + \lambda^{{\prime},*}_7\Big)Z_{{l 2}}^{H} \Big)\nonumber \\ 
 &+\Big(4 \lambda_2''  + 4 \lambda_2''^*  + 6 \lambda^{\prime\prime}_3  + \lambda_1'' + \lambda_1''^*\Big)Z_{{k 3}}^{H} Z_{{l 3}}^{H} \Big)\Big)\nonumber \\ 
 &+Z_{{i 2}}^{H} \Big(2 Z_{{j 3}}^{H} \Big(Z_{{k 3}}^{H} \Big(2 \Big(\lambda^{\prime}_2 + \lambda^{\prime}_5 + \lambda^{{\prime},*}_5\Big)Z_{{l 2}}^{H}  + \Big(\lambda^{\prime}_3 + \lambda^{\prime}_6 + \lambda^{\prime}_7 + \lambda^{{\prime},*}_3 + \lambda^{{\prime},*}_6 + \lambda^{{\prime},*}_7\Big)Z_{{l 1}}^{H} \Big)\nonumber \\ 
 &+\Big(2 \Big(\lambda^{\prime}_2 + \lambda^{\prime}_5 + \lambda^{{\prime},*}_5\Big)Z_{{k 2}}^{H}  + \Big(\lambda^{\prime}_3 + \lambda^{\prime}_6 + \lambda^{\prime}_7 + \lambda^{{\prime},*}_3 + \lambda^{{\prime},*}_6 + \lambda^{{\prime},*}_7\Big)Z_{{k 1}}^{H} \Big)Z_{{l 3}}^{H} \Big)\nonumber \\ 
 &+Z_{{j 2}}^{H} \Big(3 Z_{{k 2}}^{H} \Big(2 \lambda_2 Z_{{l 2}}^{H}  + \Big(\lambda_7 + \lambda_7^*\Big)Z_{{l 1}}^{H} \Big)+Z_{{k 1}}^{H} \Big(\Big(2 \lambda_3  + 2 \lambda_4  + \lambda_5 + \lambda_5^*\Big)Z_{{l 1}}^{H}  + 3 \Big(\lambda_7 + \lambda_7^*\Big)Z_{{l 2}}^{H} \Big)\nonumber \\ 
 &+4 \Big(\lambda^{\prime}_2 + \lambda^{\prime}_5 + \lambda^{{\prime},*}_5\Big)Z_{{k 3}}^{H} Z_{{l 3}}^{H} \Big)\nonumber \\ 
 &+Z_{{j 1}}^{H} \Big(Z_{{k 1}}^{H} \Big(\Big(2 \lambda_3  + 2 \lambda_4  + \lambda_5 + \lambda_5^*\Big)Z_{{l 2}}^{H}  + 3 \Big(\lambda_6 + \lambda_6^*\Big)Z_{{l 1}}^{H} \Big)+Z_{{k 2}}^{H} \Big(\Big(2 \lambda_3  + 2 \lambda_4  + \lambda_5 + \lambda_5^*\Big)Z_{{l 1}}^{H}  + 3 \Big(\lambda_7 + \lambda_7^*\Big)Z_{{l 2}}^{H} \Big)\nonumber \\ 
 &+2 \Big(\lambda^{\prime}_3 + \lambda^{\prime}_6 + \lambda^{\prime}_7 + \lambda^{{\prime},*}_3 + \lambda^{{\prime},*}_6 + \lambda^{{\prime},*}_7\Big)Z_{{k 3}}^{H} Z_{{l 3}}^{H} \Big)\Big)\nonumber \\ 
 &+Z_{{i 1}}^{H} \Big(2 Z_{{j 3}}^{H} \Big(Z_{{k 3}}^{H} \Big(2 \Big(\lambda^{\prime}_1 + \lambda^{\prime}_4 + \lambda^{{\prime},*}_4\Big)Z_{{l 1}}^{H}  + \Big(\lambda^{\prime}_3 + \lambda^{\prime}_6 + \lambda^{\prime}_7 + \lambda^{{\prime},*}_3 + \lambda^{{\prime},*}_6 + \lambda^{{\prime},*}_7\Big)Z_{{l 2}}^{H} \Big)\nonumber \\ 
 &+\Big(2 \Big(\lambda^{\prime}_1 + \lambda^{\prime}_4 + \lambda^{{\prime},*}_4\Big)Z_{{k 1}}^{H}  + \Big(\lambda^{\prime}_3 + \lambda^{\prime}_6 + \lambda^{\prime}_7 + \lambda^{{\prime},*}_3 + \lambda^{{\prime},*}_6 + \lambda^{{\prime},*}_7\Big)Z_{{k 2}}^{H} \Big)Z_{{l 3}}^{H} \Big)\nonumber \\ 
 &+Z_{{j 1}}^{H} \Big(Z_{{k 2}}^{H} \Big(\Big(2 \lambda_3  + 2 \lambda_4  + \lambda_5 + \lambda_5^*\Big)Z_{{l 2}}^{H}  + 3 \Big(\lambda_6 + \lambda_6^*\Big)Z_{{l 1}}^{H} \Big)+3 Z_{{k 1}}^{H} \Big(2 \lambda_1 Z_{{l 1}}^{H}  + \Big(\lambda_6 + \lambda_6^*\Big)Z_{{l 2}}^{H} \Big)\nonumber \\ 
 &+4 \Big(\lambda^{\prime}_1 + \lambda^{\prime}_4 + \lambda^{{\prime},*}_4\Big)Z_{{k 3}}^{H} Z_{{l 3}}^{H} \Big)\nonumber \\ 
 &+Z_{{j 2}}^{H} \Big(Z_{{k 1}}^{H} \Big(\Big(2 \lambda_3  + 2 \lambda_4  + \lambda_5 + \lambda_5^*\Big)Z_{{l 2}}^{H}  + 3 \Big(\lambda_6 + \lambda_6^*\Big)Z_{{l 1}}^{H} \Big)+Z_{{k 2}}^{H} \Big(\Big(2 \lambda_3  + 2 \lambda_4  + \lambda_5 + \lambda_5^*\Big)Z_{{l 1}}^{H}  + 3 \Big(\lambda_7 + \lambda_7^*\Big)Z_{{l 2}}^{H} \Big)\nonumber \\ 
 &+2 \Big(\lambda^{\prime}_3 + \lambda^{\prime}_6 + \lambda^{\prime}_7 + \lambda^{{\prime},*}_3 + \lambda^{{\prime},*}_6 + \lambda^{{\prime},*}_7\Big)Z_{{k 3}}^{H} Z_{{l 3}}^{H} \Big)\Big)\Big)\end{align} 
\hrule 
\begin{center} 
\begin{fmffile}{Diagrams/FeynDia13} 
\fmfframe(20,20)(20,20){ 
\begin{fmfgraph*}(75,75) 
\fmfleft{l1,l2}
\fmfright{r1,r2}
\fmf{dashes}{l1,v1}
\fmf{dashes}{r1,v1}
\fmf{scalar}{r2,v1}
\fmf{scalar}{v1,l2}
\fmflabel{$h_{{i}}$}{l1}
\fmflabel{$h_{{j}}$}{r1}
\fmflabel{$H^-_{{k}}$}{r2}
\fmflabel{$H^+_{{l}}$}{l2}
\end{fmfgraph*}} 
\end{fmffile} 
\end{center}  
\begin{align} 
 &-\frac{i}{2} \Big(4 Z_{{i 3}}^{H} Z_{{j 3}}^{H} \Big(Z_{{k 1}}^{+} \Big(\Big(\lambda^{\prime}_1 + \lambda^{\prime}_4 + \lambda^{{\prime},*}_4\Big)Z_{{l 1}}^{+}  + \Big(\lambda^{\prime}_3 + \lambda^{\prime}_6 + \lambda^{{\prime},*}_7\Big)Z_{{l 2}}^{+} \Big) + Z_{{k 2}}^{+} \Big(\Big(\lambda^{\prime}_2 + \lambda^{\prime}_5 + \lambda^{{\prime},*}_5\Big)Z_{{l 2}}^{+}  + \Big(\lambda^{\prime}_7 + \lambda^{{\prime},*}_3 + \lambda^{{\prime},*}_6\Big)Z_{{l 1}}^{+} \Big)\Big)\nonumber \\ 
 &+Z_{{i 2}}^{H} \Big(2 Z_{{j 2}}^{H} \Big(Z_{{k 1}}^{+} \Big(\lambda_3 Z_{{l 1}}^{+}  + \lambda_7 Z_{{l 2}}^{+} \Big) + Z_{{k 2}}^{+} \Big(\lambda_2 Z_{{l 2}}^{+}  + \lambda_7^* Z_{{l 1}}^{+} \Big)\Big)\nonumber \\ 
 &+Z_{{j 1}}^{H} \Big(Z_{{k 1}}^{+} \Big(\Big(\lambda_4 + \lambda_5^*\Big)Z_{{l 2}}^{+}  + \Big(\lambda_6 + \lambda_6^*\Big)Z_{{l 1}}^{+} \Big) + Z_{{k 2}}^{+} \Big(\Big(\lambda_4 + \lambda_5\Big)Z_{{l 1}}^{+}  + \Big(\lambda_7 + \lambda_7^*\Big)Z_{{l 2}}^{+} \Big)\Big)\Big)\nonumber \\ 
 &+Z_{{i 1}}^{H} \Big(2 Z_{{j 1}}^{H} \Big(Z_{{k 1}}^{+} \Big(\lambda_1 Z_{{l 1}}^{+}  + \lambda_6 Z_{{l 2}}^{+} \Big) + Z_{{k 2}}^{+} \Big(\lambda_3 Z_{{l 2}}^{+}  + \lambda_6^* Z_{{l 1}}^{+} \Big)\Big)\nonumber \\ 
 &+Z_{{j 2}}^{H} \Big(Z_{{k 1}}^{+} \Big(\Big(\lambda_4 + \lambda_5^*\Big)Z_{{l 2}}^{+}  + \Big(\lambda_6 + \lambda_6^*\Big)Z_{{l 1}}^{+} \Big) + Z_{{k 2}}^{+} \Big(\Big(\lambda_4 + \lambda_5\Big)Z_{{l 1}}^{+}  + \Big(\lambda_7 + \lambda_7^*\Big)Z_{{l 2}}^{+} \Big)\Big)\Big)\Big)\end{align} 
\hrule 
\begin{center} 
\begin{fmffile}{Diagrams/FeynDia14} 
\fmfframe(20,20)(20,20){ 
\begin{fmfgraph*}(75,75) 
\fmfleft{l1,l2}
\fmfright{r1,r2}
\fmf{scalar}{l1,v1}
\fmf{scalar}{r1,v1}
\fmf{scalar}{v1,r2}
\fmf{scalar}{v1,l2}
\fmflabel{$H^-_{{i}}$}{l1}
\fmflabel{$H^-_{{j}}$}{r1}
\fmflabel{$H^+_{{k}}$}{r2}
\fmflabel{$H^+_{{l}}$}{l2}
\end{fmfgraph*}} 
\end{fmffile} 
\end{center}  
\begin{align} 
 &-i \Big(Z_{{i 1}}^{+} \Big(Z_{{j 2}}^{+} \Big(2 \lambda_6^* Z_{{k 1}}^{+} Z_{{l 1}}^{+}  + \Big(\lambda_3 + \lambda_4\Big)Z_{{k 1}}^{+} Z_{{l 2}}^{+}  + Z_{{k 2}}^{+} \Big(2 \lambda_7 Z_{{l 2}}^{+}  + \Big(\lambda_3 + \lambda_4\Big)Z_{{l 1}}^{+} \Big)\Big)\nonumber \\ 
 &+2 Z_{{j 1}}^{+} \Big(Z_{{k 1}}^{+} \Big(\lambda_1 Z_{{l 1}}^{+}  + \lambda_6 Z_{{l 2}}^{+} \Big) + Z_{{k 2}}^{+} \Big(\lambda_5^* Z_{{l 2}}^{+}  + \lambda_6 Z_{{l 1}}^{+} \Big)\Big)\Big)\nonumber \\ 
 &+Z_{{i 2}}^{+} \Big(2 \lambda_6^* Z_{{j 1}}^{+} Z_{{k 1}}^{+} Z_{{l 1}}^{+} +Z_{{j 1}}^{+} \Big(\Big(\lambda_3 + \lambda_4\Big)Z_{{k 1}}^{+} Z_{{l 2}}^{+}  + Z_{{k 2}}^{+} \Big(2 \lambda_7 Z_{{l 2}}^{+}  + \Big(\lambda_3 + \lambda_4\Big)Z_{{l 1}}^{+} \Big)\Big)\nonumber \\ 
 &+2 Z_{{j 2}}^{+} \Big(Z_{{k 1}}^{+} \Big(\lambda_5 Z_{{l 1}}^{+}  + \lambda_7^* Z_{{l 2}}^{+} \Big) + Z_{{k 2}}^{+} \Big(\lambda_2 Z_{{l 2}}^{+}  + \lambda_7^* Z_{{l 1}}^{+} \Big)\Big)\Big)\Big)\end{align} 
\hrule 
