\begin{center} 
\begin{fmffile}{Diagrams/FeynDia0} 
\fmfframe(20,20)(20,20){ 
\begin{fmfgraph*}(75,75) 
\fmfleft{l1}
\fmfright{r1,r2}
\fmf{dashes}{l1,v1}
\fmf{dashes}{r1,v1}
\fmf{dashes}{r2,v1}
\fmflabel{$A^0_{{i}}$}{l1}
\fmflabel{$A^0_{{j}}$}{r1}
\fmflabel{$A^0_{{k}}$}{r2}
\end{fmfgraph*}} 
\end{fmffile} 
\end{center}  
\begin{align} 
 &\frac{1}{2} \Big(Z_{{i 1}}^{A} \Big(Z_{{j 3}}^{A} \Big(2 \Big(2 \lambda^{\prime}_4 v_S  -2 v_S \lambda^{{\prime},*}_4  - \mu_{11}^*  + \mu_{11}\Big)Z_{{k 1}}^{A} \nonumber \\ 
 &+\Big(2 \lambda^{\prime}_6 v_S  + 2 \lambda^{\prime}_7 v_S  -2 v_S \lambda^{{\prime},*}_6  -2 v_S \lambda^{{\prime},*}_7  - \mu_{12}^*  - \mu_{21}^*  + \mu_{12} + \mu_{21}\Big)Z_{{k 2}}^{A} \nonumber \\ 
 &+2 v_2 \Big(- \lambda^{\prime}_3  - \lambda^{{\prime},*}_6  - \lambda^{\prime}_7  + \lambda^{\prime}_6 + \lambda^{{\prime},*}_3 + \lambda^{{\prime},*}_7\Big)Z_{{k 3}}^{A} \Big)\nonumber \\ 
 &+Z_{{j 1}}^{A} \Big(3 v_2 \Big(- \lambda_6  + \lambda_6^*\Big)Z_{{k 1}}^{A} +\Big(\lambda_5 v_2  + \lambda_6 v_1  - v_1 \lambda_6^*  - v_2 \lambda_5^* \Big)Z_{{k 2}}^{A} \nonumber \\ 
 &+2 \Big(2 \lambda^{\prime}_4 v_S  -2 v_S \lambda^{{\prime},*}_4  - \mu_{11}^*  + \mu_{11}\Big)Z_{{k 3}}^{A} \Big)\nonumber \\ 
 &+Z_{{j 2}}^{A} \Big(\Big(\lambda_5 v_2  + \lambda_6 v_1  - v_1 \lambda_6^*  - v_2 \lambda_5^* \Big)Z_{{k 1}}^{A} +\Big(- \lambda_5 v_1  - \lambda_7 v_2  + v_1 \lambda_5^*  + v_2 \lambda_7^* \Big)Z_{{k 2}}^{A} \nonumber \\ 
 &+\Big(2 \lambda^{\prime}_6 v_S  + 2 \lambda^{\prime}_7 v_S  -2 v_S \lambda^{{\prime},*}_6  -2 v_S \lambda^{{\prime},*}_7  - \mu_{12}^*  - \mu_{21}^*  + \mu_{12} + \mu_{21}\Big)Z_{{k 3}}^{A} \Big)\Big)\nonumber \\ 
 &+Z_{{i 2}}^{A} \Big(Z_{{j 3}}^{A} \Big(\Big(2 \lambda^{\prime}_6 v_S  + 2 \lambda^{\prime}_7 v_S  -2 v_S \lambda^{{\prime},*}_6  -2 v_S \lambda^{{\prime},*}_7  - \mu_{12}^*  - \mu_{21}^*  + \mu_{12} + \mu_{21}\Big)Z_{{k 1}}^{A} \nonumber \\ 
 &+2 \Big(2 \lambda^{\prime}_5 v_S  -2 v_S \lambda^{{\prime},*}_5  - \mu_{22}^*  + \mu_{22}\Big)Z_{{k 2}}^{A} +2 v_1 \Big(- \lambda^{{\prime},*}_3  - \lambda^{\prime}_6  - \lambda^{{\prime},*}_7  + \lambda^{\prime}_3 + \lambda^{\prime}_7 + \lambda^{{\prime},*}_6\Big)Z_{{k 3}}^{A} \Big)\nonumber \\ 
 &+Z_{{j 1}}^{A} \Big(\Big(\lambda_5 v_2  + \lambda_6 v_1  - v_1 \lambda_6^*  - v_2 \lambda_5^* \Big)Z_{{k 1}}^{A} +\Big(- \lambda_5 v_1  - \lambda_7 v_2  + v_1 \lambda_5^*  + v_2 \lambda_7^* \Big)Z_{{k 2}}^{A} \nonumber \\ 
 &+\Big(2 \lambda^{\prime}_6 v_S  + 2 \lambda^{\prime}_7 v_S  -2 v_S \lambda^{{\prime},*}_6  -2 v_S \lambda^{{\prime},*}_7  - \mu_{12}^*  - \mu_{21}^*  + \mu_{12} + \mu_{21}\Big)Z_{{k 3}}^{A} \Big)\nonumber \\ 
 &+Z_{{j 2}}^{A} \Big(\Big(- \lambda_5 v_1  - \lambda_7 v_2  + v_1 \lambda_5^*  + v_2 \lambda_7^* \Big)Z_{{k 1}}^{A} +3 v_1 \Big(- \lambda_7^*  + \lambda_7\Big)Z_{{k 2}}^{A} \nonumber \\ 
 &+2 \Big(2 \lambda^{\prime}_5 v_S  -2 v_S \lambda^{{\prime},*}_5  - \mu_{22}^*  + \mu_{22}\Big)Z_{{k 3}}^{A} \Big)\Big)\nonumber \\ 
 &+Z_{{i 3}}^{A} \Big(Z_{{j 2}}^{A} \Big(\Big(2 \lambda^{\prime}_6 v_S  + 2 \lambda^{\prime}_7 v_S  -2 v_S \lambda^{{\prime},*}_6  -2 v_S \lambda^{{\prime},*}_7  - \mu_{12}^*  - \mu_{21}^*  + \mu_{12} + \mu_{21}\Big)Z_{{k 1}}^{A} \nonumber \\ 
 &+2 \Big(2 \lambda^{\prime}_5 v_S  -2 v_S \lambda^{{\prime},*}_5  - \mu_{22}^*  + \mu_{22}\Big)Z_{{k 2}}^{A} +2 v_1 \Big(- \lambda^{{\prime},*}_3  - \lambda^{\prime}_6  - \lambda^{{\prime},*}_7  + \lambda^{\prime}_3 + \lambda^{\prime}_7 + \lambda^{{\prime},*}_6\Big)Z_{{k 3}}^{A} \Big)\nonumber \\ 
 &+Z_{{j 1}}^{A} \Big(2 \Big(2 \lambda^{\prime}_4 v_S  -2 v_S \lambda^{{\prime},*}_4  - \mu_{11}^*  + \mu_{11}\Big)Z_{{k 1}}^{A} \nonumber \\ 
 &+\Big(2 \lambda^{\prime}_6 v_S  + 2 \lambda^{\prime}_7 v_S  -2 v_S \lambda^{{\prime},*}_6  -2 v_S \lambda^{{\prime},*}_7  - \mu_{12}^*  - \mu_{21}^*  + \mu_{12} + \mu_{21}\Big)Z_{{k 2}}^{A} \nonumber \\ 
 &+2 v_2 \Big(- \lambda^{\prime}_3  - \lambda^{{\prime},*}_6  - \lambda^{\prime}_7  + \lambda^{\prime}_6 + \lambda^{{\prime},*}_3 + \lambda^{{\prime},*}_7\Big)Z_{{k 3}}^{A} \Big)\nonumber \\ 
 &-2 Z_{{j 3}}^{A} \Big(v_2 \Big(- \lambda^{{\prime},*}_3  - \lambda^{\prime}_6  - \lambda^{{\prime},*}_7  + \lambda^{\prime}_3 + \lambda^{\prime}_7 + \lambda^{{\prime},*}_6\Big)Z_{{k 1}}^{A} +v_1 \Big(- \lambda^{\prime}_3  - \lambda^{{\prime},*}_6  - \lambda^{\prime}_7  + \lambda^{\prime}_6 + \lambda^{{\prime},*}_3 + \lambda^{{\prime},*}_7\Big)Z_{{k 2}}^{A} \nonumber \\ 
 &+\Big(-2 \lambda_2'' v_S  + 2 v_S \lambda_2''^*  -3 \mu_{S2}  + 3 \mu_{S2}^*  + \lambda_1'' v_S  - \mu_{S1}^*  - v_S \lambda_1''^*  + \mu_{S1}\Big)Z_{{k 3}}^{A} \Big)\Big)\Big)\end{align} 
\hrule 
\begin{center} 
\begin{fmffile}{Diagrams/FeynDia1} 
\fmfframe(20,20)(20,20){ 
\begin{fmfgraph*}(75,75) 
\fmfleft{l1}
\fmfright{r1,r2}
\fmf{dashes}{l1,v1}
\fmf{dashes}{r1,v1}
\fmf{dashes}{r2,v1}
\fmflabel{$A^0_{{i}}$}{l1}
\fmflabel{$A^0_{{j}}$}{r1}
\fmflabel{$h_{{k}}$}{r2}
\end{fmfgraph*}} 
\end{fmffile} 
\end{center}  
\begin{align} 
 &-\frac{i}{2} \Big(Z_{{i 1}}^{A} \Big(Z_{{j 3}}^{A} \Big(\Big(2 \lambda^{\prime}_6 v_S  -2 \lambda^{\prime}_7 v_S  + 2 v_S \lambda^{{\prime},*}_6  -2 v_S \lambda^{{\prime},*}_7  - \mu_{21}  - \mu_{21}^*  + \mu_{12} + \mu_{12}^*\Big)Z_{{k 2}}^{H} \nonumber \\ 
 &+2 v_2 \Big(- \lambda^{{\prime},*}_7  - \lambda^{\prime}_7  + \lambda^{\prime}_6 + \lambda^{{\prime},*}_6\Big)Z_{{k 3}}^{H} \Big)\nonumber \\ 
 &+Z_{{j 1}}^{A} \Big(\Big(2 \lambda_1 v_1  + \lambda_6 v_2  + v_2 \lambda_6^* \Big)Z_{{k 1}}^{H} +\Big(2 \lambda_3 v_2  + 2 \lambda_4 v_2  - \lambda_5 v_2  + \lambda_6 v_1  + v_1 \lambda_6^*  - v_2 \lambda_5^* \Big)Z_{{k 2}}^{H} \nonumber \\ 
 &+2 \Big(2 \lambda^{\prime}_1 v_S  + 2 \lambda^{\prime}_4 v_S  + 2 v_S \lambda^{{\prime},*}_4  + \mu_{11} + \mu_{11}^*\Big)Z_{{k 3}}^{H} \Big)\nonumber \\ 
 &+Z_{{j 2}}^{A} \Big(\Big(\lambda_5 v_2  + \lambda_6 v_1  + v_1 \lambda_6^*  + v_2 \lambda_5^* \Big)Z_{{k 1}}^{H} +\Big(\lambda_5 v_1  + \lambda_7 v_2  + v_1 \lambda_5^*  + v_2 \lambda_7^* \Big)Z_{{k 2}}^{H} \nonumber \\ 
 &+\Big(2 \lambda^{\prime}_3 v_S  + 2 \lambda^{\prime}_6 v_S  + 2 \lambda^{\prime}_7 v_S  + 2 v_S \lambda^{{\prime},*}_3  + 2 v_S \lambda^{{\prime},*}_6  + 2 v_S \lambda^{{\prime},*}_7  + \mu_{12} + \mu_{21} + \mu_{12}^* + \mu_{21}^*\Big)Z_{{k 3}}^{H} \Big)\Big)\nonumber \\ 
 &+Z_{{i 2}}^{A} \Big(Z_{{j 3}}^{A} \Big(\Big(-2 \lambda^{\prime}_6 v_S  + 2 \lambda^{\prime}_7 v_S  -2 v_S \lambda^{{\prime},*}_6  + 2 v_S \lambda^{{\prime},*}_7  - \mu_{12}  - \mu_{12}^*  + \mu_{21} + \mu_{21}^*\Big)Z_{{k 1}}^{H} \nonumber \\ 
 &+2 v_1 \Big(- \lambda^{{\prime},*}_6  - \lambda^{\prime}_6  + \lambda^{\prime}_7 + \lambda^{{\prime},*}_7\Big)Z_{{k 3}}^{H} \Big)\nonumber \\ 
 &+Z_{{j 1}}^{A} \Big(\Big(\lambda_5 v_2  + \lambda_6 v_1  + v_1 \lambda_6^*  + v_2 \lambda_5^* \Big)Z_{{k 1}}^{H} +\Big(\lambda_5 v_1  + \lambda_7 v_2  + v_1 \lambda_5^*  + v_2 \lambda_7^* \Big)Z_{{k 2}}^{H} \nonumber \\ 
 &+\Big(2 \lambda^{\prime}_3 v_S  + 2 \lambda^{\prime}_6 v_S  + 2 \lambda^{\prime}_7 v_S  + 2 v_S \lambda^{{\prime},*}_3  + 2 v_S \lambda^{{\prime},*}_6  + 2 v_S \lambda^{{\prime},*}_7  + \mu_{12} + \mu_{21} + \mu_{12}^* + \mu_{21}^*\Big)Z_{{k 3}}^{H} \Big)\nonumber \\ 
 &+Z_{{j 2}}^{A} \Big(\Big(2 \lambda_3 v_1  + 2 \lambda_4 v_1  - \lambda_5 v_1  + \lambda_7 v_2  - v_1 \lambda_5^*  + v_2 \lambda_7^* \Big)Z_{{k 1}}^{H} +\Big(2 \lambda_2 v_2  + \lambda_7 v_1  + v_1 \lambda_7^* \Big)Z_{{k 2}}^{H} \nonumber \\ 
 &+2 \Big(2 \lambda^{\prime}_2 v_S  + 2 \lambda^{\prime}_5 v_S  + 2 v_S \lambda^{{\prime},*}_5  + \mu_{22} + \mu_{22}^*\Big)Z_{{k 3}}^{H} \Big)\Big)\nonumber \\ 
 &- Z_{{i 3}}^{A} \Big(Z_{{j 2}}^{A} \Big(\Big(2 \lambda^{\prime}_6 v_S  -2 \lambda^{\prime}_7 v_S  + 2 v_S \lambda^{{\prime},*}_6  -2 v_S \lambda^{{\prime},*}_7  - \mu_{21}  - \mu_{21}^*  + \mu_{12} + \mu_{12}^*\Big)Z_{{k 1}}^{H} \nonumber \\ 
 &+2 v_1 \Big(- \lambda^{{\prime},*}_7  - \lambda^{\prime}_7  + \lambda^{\prime}_6 + \lambda^{{\prime},*}_6\Big)Z_{{k 3}}^{H} \Big)\nonumber \\ 
 &+Z_{{j 1}}^{A} \Big(\Big(-2 \lambda^{\prime}_6 v_S  + 2 \lambda^{\prime}_7 v_S  -2 v_S \lambda^{{\prime},*}_6  + 2 v_S \lambda^{{\prime},*}_7  - \mu_{12}  - \mu_{12}^*  + \mu_{21} + \mu_{21}^*\Big)Z_{{k 2}}^{H} \nonumber \\ 
 &+2 v_2 \Big(- \lambda^{{\prime},*}_6  - \lambda^{\prime}_6  + \lambda^{\prime}_7 + \lambda^{{\prime},*}_7\Big)Z_{{k 3}}^{H} \Big)\nonumber \\ 
 &+2 Z_{{j 3}}^{A} \Big(\Big(-2 \lambda^{\prime}_1 v_1  + 2 \lambda^{\prime}_4 v_1  + 2 v_1 \lambda^{{\prime},*}_4  - \lambda^{\prime}_3 v_2  + \lambda^{\prime}_6 v_2  + \lambda^{\prime}_7 v_2  - v_2 \lambda^{{\prime},*}_3  + v_2 \lambda^{{\prime},*}_6  + v_2 \lambda^{{\prime},*}_7 \Big)Z_{{k 1}}^{H} \nonumber \\ 
 &+\Big(-2 \lambda^{\prime}_2 v_2  + 2 \lambda^{\prime}_5 v_2  + 2 v_2 \lambda^{{\prime},*}_5  - \lambda^{\prime}_3 v_1  + \lambda^{\prime}_6 v_1  + \lambda^{\prime}_7 v_1  - v_1 \lambda^{{\prime},*}_3  + v_1 \lambda^{{\prime},*}_6  + v_1 \lambda^{{\prime},*}_7 \Big)Z_{{k 2}}^{H} \nonumber \\ 
 &+\Big(-2 \lambda^{\prime\prime}_3 v_S  + \lambda_1'' v_S  - \mu_{S2}  - \mu_{S2}^*  + v_S \lambda_1''^*  + \mu_{S1} + \mu_{S1}^*\Big)Z_{{k 3}}^{H} \Big)\Big)\Big)\end{align} 
\hrule 
\begin{center} 
\begin{fmffile}{Diagrams/FeynDia2} 
\fmfframe(20,20)(20,20){ 
\begin{fmfgraph*}(75,75) 
\fmfleft{l1}
\fmfright{r1,r2}
\fmf{dashes}{l1,v1}
\fmf{dashes}{r1,v1}
\fmf{dashes}{r2,v1}
\fmflabel{$A^0_{{i}}$}{l1}
\fmflabel{$h_{{j}}$}{r1}
\fmflabel{$h_{{k}}$}{r2}
\end{fmfgraph*}} 
\end{fmffile} 
\end{center}  
\begin{align} 
 &\frac{1}{2} \Big(Z_{{i 1}}^{A} \Big(Z_{{j 1}}^{H} \Big(\Big(\lambda_5 v_2  - \lambda_6 v_1  + v_1 \lambda_6^*  - v_2 \lambda_5^* \Big)Z_{{k 2}}^{H}  + v_2 \Big(- \lambda_6  + \lambda_6^*\Big)Z_{{k 1}}^{H} \Big)\nonumber \\ 
 &+Z_{{j 3}}^{H} \Big(\Big(-2 \lambda^{\prime}_3 v_S  -2 \lambda^{\prime}_6 v_S  + 2 \lambda^{\prime}_7 v_S  + 2 v_S \lambda^{{\prime},*}_3  + 2 v_S \lambda^{{\prime},*}_6  -2 v_S \lambda^{{\prime},*}_7  - \mu_{12}  - \mu_{21}^*  + \mu_{21} + \mu_{12}^*\Big)Z_{{k 2}}^{H} \nonumber \\ 
 &+2 v_2 \Big(- \lambda^{\prime}_3  - \lambda^{\prime}_6  - \lambda^{{\prime},*}_7  + \lambda^{\prime}_7 + \lambda^{{\prime},*}_3 + \lambda^{{\prime},*}_6\Big)Z_{{k 3}}^{H} \Big)\nonumber \\ 
 &+Z_{{j 2}}^{H} \Big(\Big(\lambda_5 v_2  - \lambda_6 v_1  + v_1 \lambda_6^*  - v_2 \lambda_5^* \Big)Z_{{k 1}}^{H} +\Big(-3 \lambda_7 v_2  + 3 v_2 \lambda_7^*  + \lambda_5 v_1  - v_1 \lambda_5^* \Big)Z_{{k 2}}^{H} \nonumber \\ 
 &+\Big(-2 \lambda^{\prime}_3 v_S  -2 \lambda^{\prime}_6 v_S  + 2 \lambda^{\prime}_7 v_S  + 2 v_S \lambda^{{\prime},*}_3  + 2 v_S \lambda^{{\prime},*}_6  -2 v_S \lambda^{{\prime},*}_7  - \mu_{12}  - \mu_{21}^*  + \mu_{21} + \mu_{12}^*\Big)Z_{{k 3}}^{H} \Big)\Big)\nonumber \\ 
 &+Z_{{i 2}}^{A} \Big(Z_{{j 2}}^{H} \Big(\Big(- \lambda_5 v_1  + \lambda_7 v_2  + v_1 \lambda_5^*  - v_2 \lambda_7^* \Big)Z_{{k 1}}^{H}  + v_1 \Big(- \lambda_7^*  + \lambda_7\Big)Z_{{k 2}}^{H} \Big)\nonumber \\ 
 &+Z_{{j 3}}^{H} \Big(\Big(2 \lambda^{\prime}_3 v_S  + 2 \lambda^{\prime}_6 v_S  -2 \lambda^{\prime}_7 v_S  -2 v_S \lambda^{{\prime},*}_3  -2 v_S \lambda^{{\prime},*}_6  + 2 v_S \lambda^{{\prime},*}_7  - \mu_{12}^*  - \mu_{21}  + \mu_{12} + \mu_{21}^*\Big)Z_{{k 1}}^{H} \nonumber \\ 
 &+2 v_1 \Big(- \lambda^{{\prime},*}_3  - \lambda^{{\prime},*}_6  - \lambda^{\prime}_7  + \lambda^{\prime}_3 + \lambda^{\prime}_6 + \lambda^{{\prime},*}_7\Big)Z_{{k 3}}^{H} \Big)\nonumber \\ 
 &+Z_{{j 1}}^{H} \Big(\Big(3 \lambda_6 v_1  -3 v_1 \lambda_6^*  - \lambda_5 v_2  + v_2 \lambda_5^* \Big)Z_{{k 1}}^{H} +\Big(- \lambda_5 v_1  + \lambda_7 v_2  + v_1 \lambda_5^*  - v_2 \lambda_7^* \Big)Z_{{k 2}}^{H} \nonumber \\ 
 &+\Big(2 \lambda^{\prime}_3 v_S  + 2 \lambda^{\prime}_6 v_S  -2 \lambda^{\prime}_7 v_S  -2 v_S \lambda^{{\prime},*}_3  -2 v_S \lambda^{{\prime},*}_6  + 2 v_S \lambda^{{\prime},*}_7  - \mu_{12}^*  - \mu_{21}  + \mu_{12} + \mu_{21}^*\Big)Z_{{k 3}}^{H} \Big)\Big)\nonumber \\ 
 &+Z_{{i 3}}^{A} \Big(Z_{{j 2}}^{H} \Big(\Big(2 \lambda^{\prime}_6 v_S  + 2 \lambda^{\prime}_7 v_S  -2 v_S \lambda^{{\prime},*}_6  -2 v_S \lambda^{{\prime},*}_7  - \mu_{12}^*  - \mu_{21}^*  + \mu_{12} + \mu_{21}\Big)Z_{{k 1}}^{H} \nonumber \\ 
 &+2 \Big(2 \lambda^{\prime}_5 v_S  -2 v_S \lambda^{{\prime},*}_5  - \mu_{22}^*  + \mu_{22}\Big)Z_{{k 2}}^{H} \nonumber \\ 
 &+2 \Big(2 \lambda^{\prime}_5 v_2  -2 v_2 \lambda^{{\prime},*}_5  + \lambda^{\prime}_6 v_1  + \lambda^{\prime}_7 v_1  - v_1 \lambda^{{\prime},*}_6  - v_1 \lambda^{{\prime},*}_7 \Big)Z_{{k 3}}^{H} \Big)\nonumber \\ 
 &+Z_{{j 1}}^{H} \Big(2 \Big(2 \lambda^{\prime}_4 v_S  -2 v_S \lambda^{{\prime},*}_4  - \mu_{11}^*  + \mu_{11}\Big)Z_{{k 1}}^{H} \nonumber \\ 
 &+\Big(2 \lambda^{\prime}_6 v_S  + 2 \lambda^{\prime}_7 v_S  -2 v_S \lambda^{{\prime},*}_6  -2 v_S \lambda^{{\prime},*}_7  - \mu_{12}^*  - \mu_{21}^*  + \mu_{12} + \mu_{21}\Big)Z_{{k 2}}^{H} \nonumber \\ 
 &+2 \Big(2 \lambda^{\prime}_4 v_1  -2 v_1 \lambda^{{\prime},*}_4  + \lambda^{\prime}_6 v_2  + \lambda^{\prime}_7 v_2  - v_2 \lambda^{{\prime},*}_6  - v_2 \lambda^{{\prime},*}_7 \Big)Z_{{k 3}}^{H} \Big)\nonumber \\ 
 &+2 Z_{{j 3}}^{H} \Big(\Big(2 \lambda^{\prime}_4 v_1  -2 v_1 \lambda^{{\prime},*}_4  + \lambda^{\prime}_6 v_2  + \lambda^{\prime}_7 v_2  - v_2 \lambda^{{\prime},*}_6  - v_2 \lambda^{{\prime},*}_7 \Big)Z_{{k 1}}^{H} \nonumber \\ 
 &+\Big(2 \lambda^{\prime}_5 v_2  -2 v_2 \lambda^{{\prime},*}_5  + \lambda^{\prime}_6 v_1  + \lambda^{\prime}_7 v_1  - v_1 \lambda^{{\prime},*}_6  - v_1 \lambda^{{\prime},*}_7 \Big)Z_{{k 2}}^{H} \nonumber \\ 
 &+\Big(2 \lambda_2'' v_S  -2 v_S \lambda_2''^*  + \lambda_1'' v_S  - \mu_{S1}^*  - \mu_{S2}^*  - v_S \lambda_1''^*  + \mu_{S1} + \mu_{S2}\Big)Z_{{k 3}}^{H} \Big)\Big)\Big)\end{align} 
\hrule 
\begin{center} 
\begin{fmffile}{Diagrams/FeynDia3} 
\fmfframe(20,20)(20,20){ 
\begin{fmfgraph*}(75,75) 
\fmfleft{l1}
\fmfright{r1,r2}
\fmf{dashes}{l1,v1}
\fmf{scalar}{r1,v1}
\fmf{scalar}{v1,r2}
\fmflabel{$A^0_{{i}}$}{l1}
\fmflabel{$H^-_{{j}}$}{r1}
\fmflabel{$H^+_{{k}}$}{r2}
\end{fmfgraph*}} 
\end{fmffile} 
\end{center}  
\begin{align} 
 &\frac{1}{2} \Big(v_1 Z_{{i 2}}^{A} \Big(Z_{{j 1}}^{+} \Big(\Big(- \lambda_4  + \lambda_5^*\Big)Z_{{k 2}}^{+}  + \Big(- \lambda_6^*  + \lambda_6\Big)Z_{{k 1}}^{+} \Big) + Z_{{j 2}}^{+} \Big(\Big(- \lambda_5  + \lambda_4\Big)Z_{{k 1}}^{+}  + \Big(- \lambda_7^*  + \lambda_7\Big)Z_{{k 2}}^{+} \Big)\Big)\nonumber \\ 
 &+v_2 Z_{{i 1}}^{A} \Big(Z_{{j 1}}^{+} \Big(\Big(- \lambda_5^*  + \lambda_4\Big)Z_{{k 2}}^{+}  + \Big(- \lambda_6  + \lambda_6^*\Big)Z_{{k 1}}^{+} \Big) + Z_{{j 2}}^{+} \Big(\Big(- \lambda_4  + \lambda_5\Big)Z_{{k 1}}^{+}  + \Big(- \lambda_7  + \lambda_7^*\Big)Z_{{k 2}}^{+} \Big)\Big)\nonumber \\ 
 &+2 Z_{{i 3}}^{A} \Big(Z_{{j 1}}^{+} \Big(\Big(2 \lambda^{\prime}_4 v_S  -2 v_S \lambda^{{\prime},*}_4  - \mu_{11}^*  + \mu_{11}\Big)Z_{{k 1}}^{+}  + \Big(2 \lambda^{\prime}_6 v_S  -2 v_S \lambda^{{\prime},*}_7  - \mu_{21}^*  + \mu_{12}\Big)Z_{{k 2}}^{+} \Big)\nonumber \\ 
 &+Z_{{j 2}}^{+} \Big(\Big(2 \lambda^{\prime}_5 v_S  -2 v_S \lambda^{{\prime},*}_5  - \mu_{22}^*  + \mu_{22}\Big)Z_{{k 2}}^{+}  + \Big(2 \lambda^{\prime}_7 v_S  -2 v_S \lambda^{{\prime},*}_6  - \mu_{12}^*  + \mu_{21}\Big)Z_{{k 1}}^{+} \Big)\Big)\Big)\end{align} 
\hrule 
\begin{center} 
\begin{fmffile}{Diagrams/FeynDia4} 
\fmfframe(20,20)(20,20){ 
\begin{fmfgraph*}(75,75) 
\fmfleft{l1}
\fmfright{r1,r2}
\fmf{dashes}{l1,v1}
\fmf{dashes}{r1,v1}
\fmf{dashes}{r2,v1}
\fmflabel{$h_{{i}}$}{l1}
\fmflabel{$h_{{j}}$}{r1}
\fmflabel{$h_{{k}}$}{r2}
\end{fmfgraph*}} 
\end{fmffile} 
\end{center}  
\begin{align} 
 &-\frac{i}{2} \Big(Z_{{i 1}}^{H} \Big(Z_{{j 3}}^{H} \Big(2 \Big(2 \lambda^{\prime}_1 v_S  + 2 \lambda^{\prime}_4 v_S  + 2 v_S \lambda^{{\prime},*}_4  + \mu_{11} + \mu_{11}^*\Big)Z_{{k 1}}^{H} \nonumber \\ 
 &+\Big(2 \lambda^{\prime}_3 v_S  + 2 \lambda^{\prime}_6 v_S  + 2 \lambda^{\prime}_7 v_S  + 2 v_S \lambda^{{\prime},*}_3  + 2 v_S \lambda^{{\prime},*}_6  + 2 v_S \lambda^{{\prime},*}_7  + \mu_{12} + \mu_{21} + \mu_{12}^* + \mu_{21}^*\Big)Z_{{k 2}}^{H} \nonumber \\ 
 &+2 \Big(2 \lambda^{\prime}_1 v_1  + 2 \lambda^{\prime}_4 v_1  + 2 v_1 \lambda^{{\prime},*}_4  + \lambda^{\prime}_3 v_2  + \lambda^{\prime}_6 v_2  + \lambda^{\prime}_7 v_2  + v_2 \lambda^{{\prime},*}_3  + v_2 \lambda^{{\prime},*}_6  + v_2 \lambda^{{\prime},*}_7 \Big)Z_{{k 3}}^{H} \Big)\nonumber \\ 
 &+Z_{{j 1}}^{H} \Big(3 \Big(2 \lambda_1 v_1  + \lambda_6 v_2  + v_2 \lambda_6^* \Big)Z_{{k 1}}^{H} +\Big(2 \lambda_3 v_2  + 2 \lambda_4 v_2  + 3 \lambda_6 v_1  + 3 v_1 \lambda_6^*  + \lambda_5 v_2  + v_2 \lambda_5^* \Big)Z_{{k 2}}^{H} \nonumber \\ 
 &+2 \Big(2 \lambda^{\prime}_1 v_S  + 2 \lambda^{\prime}_4 v_S  + 2 v_S \lambda^{{\prime},*}_4  + \mu_{11} + \mu_{11}^*\Big)Z_{{k 3}}^{H} \Big)\nonumber \\ 
 &+Z_{{j 2}}^{H} \Big(\Big(2 \lambda_3 v_2  + 2 \lambda_4 v_2  + 3 \lambda_6 v_1  + 3 v_1 \lambda_6^*  + \lambda_5 v_2  + v_2 \lambda_5^* \Big)Z_{{k 1}}^{H} \nonumber \\ 
 &+\Big(2 \lambda_3 v_1  + 2 \lambda_4 v_1  + 3 \lambda_7 v_2  + 3 v_2 \lambda_7^*  + \lambda_5 v_1  + v_1 \lambda_5^* \Big)Z_{{k 2}}^{H} \nonumber \\ 
 &+\Big(2 \lambda^{\prime}_3 v_S  + 2 \lambda^{\prime}_6 v_S  + 2 \lambda^{\prime}_7 v_S  + 2 v_S \lambda^{{\prime},*}_3  + 2 v_S \lambda^{{\prime},*}_6  + 2 v_S \lambda^{{\prime},*}_7  + \mu_{12} + \mu_{21} + \mu_{12}^* + \mu_{21}^*\Big)Z_{{k 3}}^{H} \Big)\Big)\nonumber \\ 
 &+Z_{{i 2}}^{H} \Big(Z_{{j 3}}^{H} \Big(\Big(2 \lambda^{\prime}_3 v_S  + 2 \lambda^{\prime}_6 v_S  + 2 \lambda^{\prime}_7 v_S  + 2 v_S \lambda^{{\prime},*}_3  + 2 v_S \lambda^{{\prime},*}_6  + 2 v_S \lambda^{{\prime},*}_7  + \mu_{12} + \mu_{21} + \mu_{12}^* + \mu_{21}^*\Big)Z_{{k 1}}^{H} \nonumber \\ 
 &+2 \Big(2 \lambda^{\prime}_2 v_S  + 2 \lambda^{\prime}_5 v_S  + 2 v_S \lambda^{{\prime},*}_5  + \mu_{22} + \mu_{22}^*\Big)Z_{{k 2}}^{H} \nonumber \\ 
 &+2 \Big(2 \lambda^{\prime}_2 v_2  + 2 \lambda^{\prime}_5 v_2  + 2 v_2 \lambda^{{\prime},*}_5  + \lambda^{\prime}_3 v_1  + \lambda^{\prime}_6 v_1  + \lambda^{\prime}_7 v_1  + v_1 \lambda^{{\prime},*}_3  + v_1 \lambda^{{\prime},*}_6  + v_1 \lambda^{{\prime},*}_7 \Big)Z_{{k 3}}^{H} \Big)\nonumber \\ 
 &+Z_{{j 1}}^{H} \Big(\Big(2 \lambda_3 v_2  + 2 \lambda_4 v_2  + 3 \lambda_6 v_1  + 3 v_1 \lambda_6^*  + \lambda_5 v_2  + v_2 \lambda_5^* \Big)Z_{{k 1}}^{H} \nonumber \\ 
 &+\Big(2 \lambda_3 v_1  + 2 \lambda_4 v_1  + 3 \lambda_7 v_2  + 3 v_2 \lambda_7^*  + \lambda_5 v_1  + v_1 \lambda_5^* \Big)Z_{{k 2}}^{H} \nonumber \\ 
 &+\Big(2 \lambda^{\prime}_3 v_S  + 2 \lambda^{\prime}_6 v_S  + 2 \lambda^{\prime}_7 v_S  + 2 v_S \lambda^{{\prime},*}_3  + 2 v_S \lambda^{{\prime},*}_6  + 2 v_S \lambda^{{\prime},*}_7  + \mu_{12} + \mu_{21} + \mu_{12}^* + \mu_{21}^*\Big)Z_{{k 3}}^{H} \Big)\nonumber \\ 
 &+Z_{{j 2}}^{H} \Big(\Big(2 \lambda_3 v_1  + 2 \lambda_4 v_1  + 3 \lambda_7 v_2  + 3 v_2 \lambda_7^*  + \lambda_5 v_1  + v_1 \lambda_5^* \Big)Z_{{k 1}}^{H} +3 \Big(2 \lambda_2 v_2  + \lambda_7 v_1  + v_1 \lambda_7^* \Big)Z_{{k 2}}^{H} \nonumber \\ 
 &+2 \Big(2 \lambda^{\prime}_2 v_S  + 2 \lambda^{\prime}_5 v_S  + 2 v_S \lambda^{{\prime},*}_5  + \mu_{22} + \mu_{22}^*\Big)Z_{{k 3}}^{H} \Big)\Big)\nonumber \\ 
 &+Z_{{i 3}}^{H} \Big(Z_{{j 2}}^{H} \Big(\Big(2 \lambda^{\prime}_3 v_S  + 2 \lambda^{\prime}_6 v_S  + 2 \lambda^{\prime}_7 v_S  + 2 v_S \lambda^{{\prime},*}_3  + 2 v_S \lambda^{{\prime},*}_6  + 2 v_S \lambda^{{\prime},*}_7  + \mu_{12} + \mu_{21} + \mu_{12}^* + \mu_{21}^*\Big)Z_{{k 1}}^{H} \nonumber \\ 
 &+2 \Big(2 \lambda^{\prime}_2 v_S  + 2 \lambda^{\prime}_5 v_S  + 2 v_S \lambda^{{\prime},*}_5  + \mu_{22} + \mu_{22}^*\Big)Z_{{k 2}}^{H} \nonumber \\ 
 &+2 \Big(2 \lambda^{\prime}_2 v_2  + 2 \lambda^{\prime}_5 v_2  + 2 v_2 \lambda^{{\prime},*}_5  + \lambda^{\prime}_3 v_1  + \lambda^{\prime}_6 v_1  + \lambda^{\prime}_7 v_1  + v_1 \lambda^{{\prime},*}_3  + v_1 \lambda^{{\prime},*}_6  + v_1 \lambda^{{\prime},*}_7 \Big)Z_{{k 3}}^{H} \Big)\nonumber \\ 
 &+Z_{{j 1}}^{H} \Big(2 \Big(2 \lambda^{\prime}_1 v_S  + 2 \lambda^{\prime}_4 v_S  + 2 v_S \lambda^{{\prime},*}_4  + \mu_{11} + \mu_{11}^*\Big)Z_{{k 1}}^{H} \nonumber \\ 
 &+\Big(2 \lambda^{\prime}_3 v_S  + 2 \lambda^{\prime}_6 v_S  + 2 \lambda^{\prime}_7 v_S  + 2 v_S \lambda^{{\prime},*}_3  + 2 v_S \lambda^{{\prime},*}_6  + 2 v_S \lambda^{{\prime},*}_7  + \mu_{12} + \mu_{21} + \mu_{12}^* + \mu_{21}^*\Big)Z_{{k 2}}^{H} \nonumber \\ 
 &+2 \Big(2 \lambda^{\prime}_1 v_1  + 2 \lambda^{\prime}_4 v_1  + 2 v_1 \lambda^{{\prime},*}_4  + \lambda^{\prime}_3 v_2  + \lambda^{\prime}_6 v_2  + \lambda^{\prime}_7 v_2  + v_2 \lambda^{{\prime},*}_3  + v_2 \lambda^{{\prime},*}_6  + v_2 \lambda^{{\prime},*}_7 \Big)Z_{{k 3}}^{H} \Big)\nonumber \\ 
 &+2 Z_{{j 3}}^{H} \Big(\Big(2 \lambda^{\prime}_1 v_1  + 2 \lambda^{\prime}_4 v_1  + 2 v_1 \lambda^{{\prime},*}_4  + \lambda^{\prime}_3 v_2  + \lambda^{\prime}_6 v_2  + \lambda^{\prime}_7 v_2  + v_2 \lambda^{{\prime},*}_3  + v_2 \lambda^{{\prime},*}_6  + v_2 \lambda^{{\prime},*}_7 \Big)Z_{{k 1}}^{H} \nonumber \\ 
 &+\Big(2 \lambda^{\prime}_2 v_2  + 2 \lambda^{\prime}_5 v_2  + 2 v_2 \lambda^{{\prime},*}_5  + \lambda^{\prime}_3 v_1  + \lambda^{\prime}_6 v_1  + \lambda^{\prime}_7 v_1  + v_1 \lambda^{{\prime},*}_3  + v_1 \lambda^{{\prime},*}_6  + v_1 \lambda^{{\prime},*}_7 \Big)Z_{{k 2}}^{H} \nonumber \\ 
 &+\Big(3 \mu_{S2}  + 3 \mu_{S2}^*  + 4 \lambda_2'' v_S  + 4 v_S \lambda_2''^*  + 6 \lambda^{\prime\prime}_3 v_S  + \lambda_1'' v_S  + v_S \lambda_1''^*  + \mu_{S1} + \mu_{S1}^*\Big)Z_{{k 3}}^{H} \Big)\Big)\Big)\end{align} 
\hrule 
\begin{center} 
\begin{fmffile}{Diagrams/FeynDia5} 
\fmfframe(20,20)(20,20){ 
\begin{fmfgraph*}(75,75) 
\fmfleft{l1}
\fmfright{r1,r2}
\fmf{dashes}{l1,v1}
\fmf{scalar}{r1,v1}
\fmf{scalar}{v1,r2}
\fmflabel{$h_{{i}}$}{l1}
\fmflabel{$H^-_{{j}}$}{r1}
\fmflabel{$H^+_{{k}}$}{r2}
\end{fmfgraph*}} 
\end{fmffile} 
\end{center}  
\begin{align} 
 &-\frac{i}{2} \Big(Z_{{i 2}}^{H} \Big(Z_{{j 1}}^{+} \Big(\Big(2 \lambda_3 v_2  + \lambda_6 v_1  + v_1 \lambda_6^* \Big)Z_{{k 1}}^{+}  + \Big(2 \lambda_7 v_2  + \lambda_4 v_1  + v_1 \lambda_5^* \Big)Z_{{k 2}}^{+} \Big)\nonumber \\ 
 &+Z_{{j 2}}^{+} \Big(\Big(2 \lambda_2 v_2  + \lambda_7 v_1  + v_1 \lambda_7^* \Big)Z_{{k 2}}^{+}  + \Big(2 v_2 \lambda_7^*  + \Big(\lambda_4 + \lambda_5\Big)v_1 \Big)Z_{{k 1}}^{+} \Big)\Big)\nonumber \\ 
 &+Z_{{i 1}}^{H} \Big(Z_{{j 1}}^{+} \Big(\Big(2 \lambda_1 v_1  + \lambda_6 v_2  + v_2 \lambda_6^* \Big)Z_{{k 1}}^{+}  + \Big(2 \lambda_6 v_1  + \lambda_4 v_2  + v_2 \lambda_5^* \Big)Z_{{k 2}}^{+} \Big)\nonumber \\ 
 &+Z_{{j 2}}^{+} \Big(\Big(2 \lambda_3 v_1  + \lambda_7 v_2  + v_2 \lambda_7^* \Big)Z_{{k 2}}^{+}  + \Big(2 v_1 \lambda_6^*  + \Big(\lambda_4 + \lambda_5\Big)v_2 \Big)Z_{{k 1}}^{+} \Big)\Big)\nonumber \\ 
 &+2 Z_{{i 3}}^{H} \Big(Z_{{j 1}}^{+} \Big(\Big(2 \lambda^{\prime}_1 v_S  + 2 \lambda^{\prime}_4 v_S  + 2 v_S \lambda^{{\prime},*}_4  + \mu_{11} + \mu_{11}^*\Big)Z_{{k 1}}^{+}  + \Big(2 \lambda^{\prime}_3 v_S  + 2 \lambda^{\prime}_6 v_S  + 2 v_S \lambda^{{\prime},*}_7  + \mu_{12} + \mu_{21}^*\Big)Z_{{k 2}}^{+} \Big)\nonumber \\ 
 &+Z_{{j 2}}^{+} \Big(\Big(2 \lambda^{\prime}_2 v_S  + 2 \lambda^{\prime}_5 v_S  + 2 v_S \lambda^{{\prime},*}_5  + \mu_{22} + \mu_{22}^*\Big)Z_{{k 2}}^{+}  + \Big(2 \lambda^{\prime}_7 v_S  + 2 v_S \lambda^{{\prime},*}_3  + 2 v_S \lambda^{{\prime},*}_6  + \mu_{21} + \mu_{12}^*\Big)Z_{{k 1}}^{+} \Big)\Big)\Big)\end{align} 
\hrule 
